Prove wp_deletionFinalizersForGarbageCollection

src/proof/kubernetes_model/common_delete.v
@@ -7,8 +7,1807 @@ From New.proof.kubernetes_model Require Export common.
 Section proof.
 Context `{hG: !heapGS Σ} `{!ffi_semantics _ _}.
 Context {sem : go.Semantics} {package_sem : apimodel.Assumptions}.
-Context `{!kubernetesModelG Σ}.
 Local Set Default Proof Using "All".
+
+Definition delete_preconditions_match (options : DeleteOptionsV.t) (m : ObjectMetaV.t) : Prop :=
+  match options.(DeleteOptionsV.Preconditions') with
+  | None => True
+  | Some preconditions =>
+      (match preconditions.(PreconditionsV.UID') with
+       | Some uid => uid = m.(ObjectMetaV.UID')
+       | None => True
+       end) ∧
+      (match preconditions.(PreconditionsV.ResourceVersion') with
+       | Some rv => rv = m.(ObjectMetaV.ResourceVersion')
+       | None => True
+       end)
+  end.
+
+#[global] Instance delete_preconditions_match_dec options m :
+  Decision (delete_preconditions_match options m).
+Proof.
+  unfold delete_preconditions_match.
+  destruct options.(DeleteOptionsV.Preconditions') as [preconditions|].
+  - destruct preconditions.(PreconditionsV.UID') as [uid|];
+      destruct preconditions.(PreconditionsV.ResourceVersion') as [rv|];
+      simpl.
+    + destruct (decide (uid = m.(ObjectMetaV.UID'))) as [Huid|Huid];
+        destruct (decide (rv = m.(ObjectMetaV.ResourceVersion'))) as [Hrv|Hrv].
+      * left. split; assumption.
+      * right. intros [_ Hrv']. contradiction.
+      * right. intros [Huid' _]. contradiction.
+      * right. intros [Huid' _]. contradiction.
+    + destruct (decide (uid = m.(ObjectMetaV.UID'))) as [Huid|Huid].
+      * left. split; [assumption|done].
+      * right. intros [Huid' _]. contradiction.
+    + destruct (decide (rv = m.(ObjectMetaV.ResourceVersion'))) as [Hrv|Hrv].
+      * left. split; [done|assumption].
+      * right. intros [_ Hrv']. contradiction.
+    + left. done.
+  - left. done.
+Qed.
+
+(* [ValidateDeleteOptions] is part of the untranslated Kubernetes validation
+   package.  [DeleteOptionsV.valid] is its pure-model counterpart. *)
+Axiom ErrorList_underlying_slice :
+  field.ErrorList ↓u go.SliceType (go.PointerType field.Error).
+#[local] Existing Instance ErrorList_underlying_slice.
+
+Axiom wp_ValidateDeleteOptions_valid : ∀ l options dq,
+  {{{ is_pkg_init apimodel ∗
+      DeleteOptionsV.deepown_l l options dq ∗
+      ⌜ DeleteOptionsV.valid options ⌝
+  }}}
+    @! v1_validation.ValidateDeleteOptions #l
+  {{{ (errs : field.ErrorList.t), RET #errs;
+      ⌜ (#errs : val) = #slice.nil ⌝ ∗
+      DeleteOptionsV.deepown_l l options dq
+  }}}.
+
+Lemma wp_validateDeleteOptions l options dq :
+  {{{ is_pkg_init apimodel ∗
+      "Hdeepown_l" ∷ DeleteOptionsV.deepown_l l options dq ∗
+      "%Hvalid" ∷ ⌜ DeleteOptionsV.valid options ⌝
+  }}}
+    @! apimodel.validateDeleteOptions #l
+  {{{ RET #interface.nil;
+      DeleteOptionsV.deepown_l l options dq
+  }}}.
+Proof.
+  wp_start as "H".
+  iNamed "H".
+  wp_auto.
+  wp_apply (wp_ValidateDeleteOptions_valid with "[$Hdeepown_l]").
+  { iFrame "#". done. }
+  iIntros (errs) "(%Herrs_nil & Hdeepown_l)".
+  wp_auto.
+  rewrite Herrs_nil.
+  wp_auto.
+  iApply "HΦ".
+  iFrame.
+Qed.
+
+Lemma wp_validateDeletePreconditions i l m options_l options dq (kind : go_string) :
+  {{{ is_pkg_init apimodel ∗
+      "%Hi" ∷ ⌜ i = interface.mk (go.PointerType v1.ObjectMeta) #l ⌝ ∗
+      "Hdeepown_m_l" ∷ ObjectMetaV.deepown_l l m dq ∗
+      "Hdeepown_options_l" ∷ DeleteOptionsV.deepown_l options_l options dq
+  }}}
+    @! apimodel.validateDeletePreconditions #(interface.ok i) #options_l #kind
+  {{{ err, RET #err;
+      ⌜ delete_preconditions_match options m ∧ err = interface.nil
+        ∨
+        ¬ delete_preconditions_match options m ∧
+          err ≠ interface.nil ∧
+          conflict_error err ⌝ ∗
+      ObjectMetaV.deepown_l l m dq ∗
+      DeleteOptionsV.deepown_l options_l options dq
+  }}}.
+Proof.
+  wp_start as "H".
+  iNamed "H". subst i.
+  iDestruct "Hdeepown_options_l" as (options_c) "[Hoptions_l Hdeepown_options]".
+  iNamed "Hdeepown_options".
+  destruct options.(DeleteOptionsV.Preconditions') as [preconditions|]
+    eqn:Hpreconditions.
+  - iDestruct "Hdeepown_preconditions_some" as (preconditions_c)
+      "[Hpreconditions_l Hdeepown_preconditions]".
+    iNamed "Hdeepown_preconditions".
+    assert (v1.DeleteOptions.Preconditions' options_c ≠ null)
+      as Hpreconditions_not_null.
+    { intros Hnull.
+      apply (proj1 Hdeepown_preconditions_none) in Hnull.
+      congruence. }
+    assert (bool_decide
+      (v1.DeleteOptions.Preconditions' options_c = null) = false)
+      as Hpreconditions_nonnull_decide.
+    { apply bool_decide_false. done. }
+    wp_auto.
+    rewrite Hpreconditions_nonnull_decide /=.
+    wp_auto.
+    destruct preconditions.(PreconditionsV.UID') as [uid|] eqn:Huid.
+    + iDestruct "Hdeepown_uid_some" as (uid_c) "[Huid_l ->]".
+      assert (v1.Preconditions.UID' preconditions_c ≠ null)
+        as Huid_not_null.
+      { intros Hnull.
+        apply (proj1 Hdeepown_uid_none) in Hnull.
+        congruence. }
+      assert (bool_decide (v1.Preconditions.UID' preconditions_c = null) = false)
+        as Huid_nonnull_decide.
+      { apply bool_decide_false. done. }
+      rewrite Huid_nonnull_decide /=.
+      wp_auto.
+      wp_apply (v1.wp_GetUID_deepown with "[$Hdeepown_m_l]").
+      iIntros "Hdeepown_m_l".
+      wp_auto.
+      wp_if_destruct.
+      * iAssert ((match preconditions.(PreconditionsV.UID') with
+          | Some uid' => ∃ uid_c',
+              v1.Preconditions.UID' preconditions_c ↦{dq} uid_c' ∗
+              ⌜ uid_c' = uid' ⌝
+          | None => True
+          end)%I) with "[Huid_l]" as "Hdeepown_uid_some".
+        { rewrite Huid /=. iExists m.(ObjectMetaV.UID'). iFrame. done. }
+        destruct preconditions.(PreconditionsV.ResourceVersion') as [rv|]
+          eqn:Hrv.
+        -- iDestruct "Hdeepown_resourceversion_some" as (rv_c) "[Hrv_l ->]".
+           assert (v1.Preconditions.ResourceVersion' preconditions_c ≠ null)
+             as Hrv_not_null.
+           { intros Hnull.
+             apply (proj1 Hdeepown_resourceversion_none) in Hnull.
+             congruence. }
+           assert (bool_decide
+             (v1.Preconditions.ResourceVersion' preconditions_c = null) = false)
+             as Hrv_nonnull_decide.
+           { apply bool_decide_false. done. }
+           rewrite Hrv_nonnull_decide /=.
+           wp_auto.
+           wp_apply (v1.wp_GetResourceVersion_deepown with "[$Hdeepown_m_l]").
+           iIntros "Hdeepown_m_l".
+           wp_auto.
+           wp_if_destruct.
+           ++ iAssert ((match preconditions.(PreconditionsV.ResourceVersion') with
+                | Some rv' => ∃ rv_c',
+                    v1.Preconditions.ResourceVersion' preconditions_c ↦{dq} rv_c' ∗
+                    ⌜ rv_c' = rv' ⌝
+                | None => True
+                end)%I) with "[Hrv_l]" as "Hdeepown_resourceversion_some".
+              { rewrite Hrv /=.
+                iExists m.(ObjectMetaV.ResourceVersion'). iFrame. done. }
+              iAssert (PreconditionsV.deepown preconditions_c preconditions dq)
+                with "[Hdeepown_uid_some Hdeepown_resourceversion_some]"
+                as "Hdeepown_preconditions".
+              { rewrite /PreconditionsV.deepown Huid Hrv /=.
+                iFrame. iPureIntro. done. }
+              iAssert ((match options.(DeleteOptionsV.Preconditions') with
+                | Some preconditions' => ∃ preconditions_c',
+                    v1.DeleteOptions.Preconditions' options_c ↦{dq} preconditions_c' ∗
+                    PreconditionsV.deepown preconditions_c' preconditions' dq
+                | None => True
+                end)%I) with "[Hpreconditions_l Hdeepown_preconditions]"
+                as "Hdeepown_preconditions_some".
+              { rewrite Hpreconditions /=.
+                iExists preconditions_c. iFrame. }
+              iAssert (DeleteOptionsV.deepown options_c options dq)
+                with "[Hdeepown_graceperiodseconds_some Hdeepown_preconditions_some Hdeepown_orphandependents_some Hdeepown_propagationpolicy_some]"
+                as "Hdeepown_options".
+              { rewrite /DeleteOptionsV.deepown Hpreconditions /=.
+                iFrame. iPureIntro. done. }
+              iApply "HΦ". iFrame. iPureIntro.
+              left. split; [|done].
+              rewrite /delete_preconditions_match Hpreconditions Huid Hrv /=.
+              done.
+           ++ wp_apply (v1.wp_GetName_deepown with "[$Hdeepown_m_l]").
+              iIntros "Hdeepown_m_l".
+              wp_auto.
+              wp_apply (v1.wp_GetResourceVersion_deepown with "[$Hdeepown_m_l]").
+              iIntros "Hdeepown_m_l".
+              wp_auto.
+              wp_apply wp_newPreconditionRVConflictError.
+              iIntros (err) "%Hconflict".
+              wp_auto.
+              iAssert ((match preconditions.(PreconditionsV.ResourceVersion') with
+                | Some rv' => ∃ rv_c',
+                    v1.Preconditions.ResourceVersion' preconditions_c ↦{dq} rv_c' ∗
+                    ⌜ rv_c' = rv' ⌝
+                | None => True
+                end)%I) with "[Hrv_l]" as "Hdeepown_resourceversion_some".
+              { rewrite Hrv /=. iExists rv. iFrame. done. }
+              iAssert (PreconditionsV.deepown preconditions_c preconditions dq)
+                with "[Hdeepown_uid_some Hdeepown_resourceversion_some]"
+                as "Hdeepown_preconditions".
+              { rewrite /PreconditionsV.deepown Huid Hrv /=.
+                iFrame. iPureIntro. done. }
+              iAssert ((match options.(DeleteOptionsV.Preconditions') with
+                | Some preconditions' => ∃ preconditions_c',
+                    v1.DeleteOptions.Preconditions' options_c ↦{dq} preconditions_c' ∗
+                    PreconditionsV.deepown preconditions_c' preconditions' dq
+                | None => True
+                end)%I) with "[Hpreconditions_l Hdeepown_preconditions]"
+                as "Hdeepown_preconditions_some".
+              { rewrite Hpreconditions /=.
+                iExists preconditions_c. iFrame. }
+              iAssert (DeleteOptionsV.deepown options_c options dq)
+                with "[Hdeepown_graceperiodseconds_some Hdeepown_preconditions_some Hdeepown_orphandependents_some Hdeepown_propagationpolicy_some]"
+                as "Hdeepown_options".
+              { rewrite /DeleteOptionsV.deepown Hpreconditions /=.
+                iFrame. iPureIntro. done. }
+              iApply "HΦ". iFrame. iPureIntro.
+              right. split.
+              { rewrite /delete_preconditions_match Hpreconditions Huid Hrv /=.
+                intuition. }
+              split; [exact (conflict_error_not_nil err Hconflict)|done].
+        -- assert (v1.Preconditions.ResourceVersion' preconditions_c = null)
+             as Hrv_null.
+           { apply (proj2 Hdeepown_resourceversion_none). done. }
+           assert (bool_decide
+             (v1.Preconditions.ResourceVersion' preconditions_c = null) = true)
+             as Hrv_null_decide.
+           { apply bool_decide_true. done. }
+           rewrite Hrv_null_decide /=.
+           wp_auto.
+           iAssert (PreconditionsV.deepown preconditions_c preconditions dq)
+             with "[Hdeepown_uid_some Hdeepown_resourceversion_some]"
+             as "Hdeepown_preconditions".
+           { rewrite /PreconditionsV.deepown Huid Hrv /=.
+             iFrame. iPureIntro. done. }
+           iAssert ((match options.(DeleteOptionsV.Preconditions') with
+             | Some preconditions' => ∃ preconditions_c',
+                 v1.DeleteOptions.Preconditions' options_c ↦{dq} preconditions_c' ∗
+                 PreconditionsV.deepown preconditions_c' preconditions' dq
+             | None => True
+             end)%I) with "[Hpreconditions_l Hdeepown_preconditions]"
+             as "Hdeepown_preconditions_some".
+           { rewrite Hpreconditions /=.
+             iExists preconditions_c. iFrame. }
+           iAssert (DeleteOptionsV.deepown options_c options dq)
+             with "[Hdeepown_graceperiodseconds_some Hdeepown_preconditions_some Hdeepown_orphandependents_some Hdeepown_propagationpolicy_some]"
+             as "Hdeepown_options".
+           { rewrite /DeleteOptionsV.deepown Hpreconditions /=.
+             iFrame. iPureIntro. done. }
+           iApply "HΦ". iFrame. iPureIntro.
+           left. split; [|done].
+           rewrite /delete_preconditions_match Hpreconditions Huid Hrv /=.
+           done.
+      * wp_apply (v1.wp_GetName_deepown with "[$Hdeepown_m_l]").
+        iIntros "Hdeepown_m_l".
+        wp_auto.
+        wp_apply (v1.wp_GetUID_deepown with "[$Hdeepown_m_l]").
+        iIntros "Hdeepown_m_l".
+        wp_auto.
+        wp_apply wp_newPreconditionUIDConflictError.
+        iIntros (err) "%Hconflict".
+        wp_auto.
+        iAssert ((match preconditions.(PreconditionsV.UID') with
+          | Some uid' => ∃ uid_c',
+              v1.Preconditions.UID' preconditions_c ↦{dq} uid_c' ∗
+              ⌜ uid_c' = uid' ⌝
+          | None => True
+          end)%I) with "[Huid_l]" as "Hdeepown_uid_some".
+        { rewrite Huid /=. iExists uid. iFrame. done. }
+        iAssert (PreconditionsV.deepown preconditions_c preconditions dq)
+          with "[Hdeepown_uid_some Hdeepown_resourceversion_some]"
+          as "Hdeepown_preconditions".
+        { rewrite /PreconditionsV.deepown Huid /=.
+          iFrame. iPureIntro. done. }
+        iAssert ((match options.(DeleteOptionsV.Preconditions') with
+          | Some preconditions' => ∃ preconditions_c',
+              v1.DeleteOptions.Preconditions' options_c ↦{dq} preconditions_c' ∗
+              PreconditionsV.deepown preconditions_c' preconditions' dq
+          | None => True
+          end)%I) with "[Hpreconditions_l Hdeepown_preconditions]"
+          as "Hdeepown_preconditions_some".
+        { rewrite Hpreconditions /=.
+          iExists preconditions_c. iFrame. }
+        iAssert (DeleteOptionsV.deepown options_c options dq)
+          with "[Hdeepown_graceperiodseconds_some Hdeepown_preconditions_some Hdeepown_orphandependents_some Hdeepown_propagationpolicy_some]"
+          as "Hdeepown_options".
+        { rewrite /DeleteOptionsV.deepown Hpreconditions /=.
+          iFrame. iPureIntro. done. }
+        iApply "HΦ". iFrame. iPureIntro.
+        right. split.
+        { rewrite /delete_preconditions_match Hpreconditions Huid /=.
+          intros [Huid_match _]. done. }
+        split; [exact (conflict_error_not_nil err Hconflict)|done].
+    + assert (v1.Preconditions.UID' preconditions_c = null) as Huid_null.
+      { apply (proj2 Hdeepown_uid_none). done. }
+      assert (bool_decide (v1.Preconditions.UID' preconditions_c = null) = true)
+        as Huid_null_decide.
+      { apply bool_decide_true. done. }
+      rewrite Huid_null_decide /=.
+      wp_auto.
+      destruct preconditions.(PreconditionsV.ResourceVersion') as [rv|]
+        eqn:Hrv.
+      * iDestruct "Hdeepown_resourceversion_some" as (rv_c) "[Hrv_l ->]".
+        assert (v1.Preconditions.ResourceVersion' preconditions_c ≠ null)
+          as Hrv_not_null.
+        { intros Hnull.
+          apply (proj1 Hdeepown_resourceversion_none) in Hnull.
+          congruence. }
+        assert (bool_decide
+          (v1.Preconditions.ResourceVersion' preconditions_c = null) = false)
+          as Hrv_nonnull_decide.
+        { apply bool_decide_false. done. }
+        rewrite Hrv_nonnull_decide /=.
+        wp_auto.
+        wp_apply (v1.wp_GetResourceVersion_deepown with "[$Hdeepown_m_l]").
+        iIntros "Hdeepown_m_l".
+        wp_auto.
+        wp_if_destruct.
+        -- iAssert ((match preconditions.(PreconditionsV.ResourceVersion') with
+             | Some rv' => ∃ rv_c',
+                 v1.Preconditions.ResourceVersion' preconditions_c ↦{dq} rv_c' ∗
+                 ⌜ rv_c' = rv' ⌝
+             | None => True
+             end)%I) with "[Hrv_l]" as "Hdeepown_resourceversion_some".
+           { rewrite Hrv /=.
+             iExists m.(ObjectMetaV.ResourceVersion'). iFrame. done. }
+           iAssert (PreconditionsV.deepown preconditions_c preconditions dq)
+             with "[Hdeepown_uid_some Hdeepown_resourceversion_some]"
+             as "Hdeepown_preconditions".
+           { rewrite /PreconditionsV.deepown Huid Hrv /=.
+             iFrame. iPureIntro. done. }
+           iAssert ((match options.(DeleteOptionsV.Preconditions') with
+             | Some preconditions' => ∃ preconditions_c',
+                 v1.DeleteOptions.Preconditions' options_c ↦{dq} preconditions_c' ∗
+                 PreconditionsV.deepown preconditions_c' preconditions' dq
+             | None => True
+             end)%I) with "[Hpreconditions_l Hdeepown_preconditions]"
+             as "Hdeepown_preconditions_some".
+           { rewrite Hpreconditions /=.
+             iExists preconditions_c. iFrame. }
+           iAssert (DeleteOptionsV.deepown options_c options dq)
+             with "[Hdeepown_graceperiodseconds_some Hdeepown_preconditions_some Hdeepown_orphandependents_some Hdeepown_propagationpolicy_some]"
+             as "Hdeepown_options".
+           { rewrite /DeleteOptionsV.deepown Hpreconditions /=.
+             iFrame. iPureIntro. done. }
+           iApply "HΦ". iFrame. iPureIntro.
+           left. split; [|done].
+           rewrite /delete_preconditions_match Hpreconditions Huid Hrv /=.
+           done.
+        -- wp_apply (v1.wp_GetName_deepown with "[$Hdeepown_m_l]").
+           iIntros "Hdeepown_m_l".
+           wp_auto.
+           wp_apply (v1.wp_GetResourceVersion_deepown with "[$Hdeepown_m_l]").
+           iIntros "Hdeepown_m_l".
+           wp_auto.
+           wp_apply wp_newPreconditionRVConflictError.
+           iIntros (err) "%Hconflict".
+           wp_auto.
+           iAssert ((match preconditions.(PreconditionsV.ResourceVersion') with
+             | Some rv' => ∃ rv_c',
+                 v1.Preconditions.ResourceVersion' preconditions_c ↦{dq} rv_c' ∗
+                 ⌜ rv_c' = rv' ⌝
+             | None => True
+             end)%I) with "[Hrv_l]" as "Hdeepown_resourceversion_some".
+           { rewrite Hrv /=. iExists rv. iFrame. done. }
+           iAssert (PreconditionsV.deepown preconditions_c preconditions dq)
+             with "[Hdeepown_uid_some Hdeepown_resourceversion_some]"
+             as "Hdeepown_preconditions".
+           { rewrite /PreconditionsV.deepown Huid Hrv /=.
+             iFrame. iPureIntro. done. }
+           iAssert ((match options.(DeleteOptionsV.Preconditions') with
+             | Some preconditions' => ∃ preconditions_c',
+                 v1.DeleteOptions.Preconditions' options_c ↦{dq} preconditions_c' ∗
+                 PreconditionsV.deepown preconditions_c' preconditions' dq
+             | None => True
+             end)%I) with "[Hpreconditions_l Hdeepown_preconditions]"
+             as "Hdeepown_preconditions_some".
+           { rewrite Hpreconditions /=.
+             iExists preconditions_c. iFrame. }
+           iAssert (DeleteOptionsV.deepown options_c options dq)
+             with "[Hdeepown_graceperiodseconds_some Hdeepown_preconditions_some Hdeepown_orphandependents_some Hdeepown_propagationpolicy_some]"
+             as "Hdeepown_options".
+           { rewrite /DeleteOptionsV.deepown Hpreconditions /=.
+             iFrame. iPureIntro. done. }
+           iApply "HΦ". iFrame. iPureIntro.
+           right. split.
+           { rewrite /delete_preconditions_match Hpreconditions Huid Hrv /=.
+             intuition. }
+           split; [exact (conflict_error_not_nil err Hconflict)|done].
+      * assert (v1.Preconditions.ResourceVersion' preconditions_c = null)
+          as Hrv_null.
+        { apply (proj2 Hdeepown_resourceversion_none). done. }
+        assert (bool_decide
+          (v1.Preconditions.ResourceVersion' preconditions_c = null) = true)
+          as Hrv_null_decide.
+        { apply bool_decide_true. done. }
+        rewrite Hrv_null_decide /=.
+        wp_auto.
+        iAssert (PreconditionsV.deepown preconditions_c preconditions dq)
+          with "[Hdeepown_uid_some Hdeepown_resourceversion_some]"
+          as "Hdeepown_preconditions".
+        { rewrite /PreconditionsV.deepown Huid Hrv /=.
+          iFrame. iPureIntro. done. }
+        iAssert ((match options.(DeleteOptionsV.Preconditions') with
+          | Some preconditions' => ∃ preconditions_c',
+              v1.DeleteOptions.Preconditions' options_c ↦{dq} preconditions_c' ∗
+              PreconditionsV.deepown preconditions_c' preconditions' dq
+          | None => True
+          end)%I) with "[Hpreconditions_l Hdeepown_preconditions]"
+          as "Hdeepown_preconditions_some".
+        { rewrite Hpreconditions /=.
+          iExists preconditions_c. iFrame. }
+        iAssert (DeleteOptionsV.deepown options_c options dq)
+          with "[Hdeepown_graceperiodseconds_some Hdeepown_preconditions_some Hdeepown_orphandependents_some Hdeepown_propagationpolicy_some]"
+          as "Hdeepown_options".
+        { rewrite /DeleteOptionsV.deepown Hpreconditions /=.
+          iFrame. iPureIntro. done. }
+        iApply "HΦ". iFrame. iPureIntro.
+        left. split; [|done].
+        rewrite /delete_preconditions_match Hpreconditions Huid Hrv /=.
+        done.
+  - assert (v1.DeleteOptions.Preconditions' options_c = null)
+      as Hpreconditions_null.
+    { apply (proj2 Hdeepown_preconditions_none). done. }
+    assert (bool_decide
+      (v1.DeleteOptions.Preconditions' options_c = null) = true)
+      as Hpreconditions_null_decide.
+    { apply bool_decide_true. done. }
+    wp_auto.
+    rewrite Hpreconditions_null_decide /=.
+    wp_auto.
+    iAssert (DeleteOptionsV.deepown options_c options dq)
+      with "[Hdeepown_graceperiodseconds_some Hdeepown_preconditions_some Hdeepown_orphandependents_some Hdeepown_propagationpolicy_some]"
+      as "Hdeepown_options".
+    { rewrite /DeleteOptionsV.deepown Hpreconditions /=.
+      iFrame. iPureIntro. done. }
+    iApply "HΦ". iFrame. iPureIntro.
+    left. split; [rewrite /delete_preconditions_match Hpreconditions /=; done|done].
+Qed.
+
+(* delete_graceful and delete_pending_graceful abstract the result of checkGracefulDelete *)
+Axiom delete_graceful : KObjectV.t -> DeleteOptionsV.t -> bool.
+Axiom delete_pending_graceful : KObjectV.t -> bool.
+Axiom delete_new_grace_period_seconds : KObjectV.t -> DeleteOptionsV.t -> option w64.
+
+Lemma wp_checkGracefulDelete i l o options_l options :
+  {{{ is_pkg_init apimodel ∗
+      "%Hvalid_i" ∷ ⌜ KObjectV.valid_interface i l o ⌝ ∗
+      "Hdeepown_l" ∷ KObjectV.deepown_l l o 1 ∗
+      "Hdeepown_options_l" ∷ DeleteOptionsV.deepown_l options_l options 1
+  }}}
+    @! apimodel.checkGracefulDelete #(interface.ok i) #options_l
+  {{{ graceful pendingGraceful options',
+      RET (#graceful, #pendingGraceful, #interface.nil);
+      KObjectV.deepown_l l o 1 ∗
+      DeleteOptionsV.deepown_l options_l options' 1 ∗
+      ⌜ pendingGraceful = true →
+        (KObjectV.objectmeta o).(ObjectMetaV.DeletionTimestamp') ≠ None ⌝ ∗
+      ⌜ graceful = delete_graceful o options ⌝ ∗
+      ⌜ pendingGraceful = delete_pending_graceful o ⌝ ∗
+      ⌜ options' = (options <| DeleteOptionsV.GracePeriodSeconds' :=
+        delete_new_grace_period_seconds o options |>) ⌝
+  }}}.
+Proof.
+Admitted.
+
+Definition delete_orphan_finalizer : go_string := "orphan"%go.
+Definition delete_foreground_finalizer : go_string := "foregroundDeletion"%go.
+
+(* [true] selects orphan deletion and [false] selects foreground deletion. *)
+Fixpoint delete_existing_gc_policy (finalizers : list go_string) : option bool :=
+  match finalizers with
+  | [] => None
+  | finalizer :: finalizers =>
+      if decide (finalizer = delete_orphan_finalizer) then Some true
+      else if decide (finalizer = delete_foreground_finalizer) then Some false
+      else delete_existing_gc_policy finalizers
+  end.
+
+Definition delete_gc_policy (m : ObjectMetaV.t) (options : DeleteOptionsV.t) :
+    option bool :=
+  match options.(DeleteOptionsV.OrphanDependents') with
+  | Some true => Some true
+  | Some false => None
+  | None =>
+      match options.(DeleteOptionsV.PropagationPolicy') with
+      | Some policy =>
+          if decide (policy = "Orphan"%go) then Some true
+          else if decide (policy = "Foreground"%go) then Some false
+          else if decide (policy = "Background"%go) then None
+          else delete_existing_gc_policy (default [] m.(ObjectMetaV.Finalizers'))
+      | None => delete_existing_gc_policy (default [] m.(ObjectMetaV.Finalizers'))
+      end
+  end.
+
+Definition delete_should_orphan_dependents m options : bool :=
+  match delete_gc_policy m options with Some true => true | _ => false end.
+
+Definition delete_should_delete_dependents m options : bool :=
+  match delete_gc_policy m options with Some false => true | _ => false end.
+
+Definition delete_finalizers_for_gc m options : list go_string :=
+  filter
+    (fun finalizer =>
+      finalizer ≠ delete_orphan_finalizer ∧
+      finalizer ≠ delete_foreground_finalizer)
+    (default [] m.(ObjectMetaV.Finalizers')) ++
+  (if delete_should_orphan_dependents m options
+   then [delete_orphan_finalizer] else []) ++
+  (if delete_should_delete_dependents m options
+   then [delete_foreground_finalizer] else []).
+
+Definition delete_finalizers_changed (old new : list go_string) : Prop :=
+  length old ≠ length new ∨ Exists (fun finalizer => finalizer ∉ old) new.
+
+#[global] Instance delete_finalizers_changed_dec old new :
+  Decision (delete_finalizers_changed old new) := _.
+
+Definition delete_should_update_finalizers m options : bool :=
+  bool_decide (delete_finalizers_changed
+    (default [] m.(ObjectMetaV.Finalizers'))
+    (delete_finalizers_for_gc m options)).
+
+Definition delete_new_finalizers m options : option (list go_string) :=
+  if delete_should_update_finalizers m options
+  then Some (delete_finalizers_for_gc m options)
+  else m.(ObjectMetaV.Finalizers').
+
+Transparent w8_word_instance.
+
+Lemma delete_orphan_finalizer_valid :
+  valid_label_name delete_orphan_finalizer.
+Proof.
+  left. split; last done.
+  rewrite /delete_orphan_finalizer /qualified_name_syntax /=.
+  repeat lazymatch goal with | |- _ ∧ _ => split end.
+  all: lazymatch goal with
+       | |- label_extended_character _ => left
+       | |- label_alphanumeric _ => idtac
+       end.
+  all: unfold label_alphanumeric;
+    first [left; cbn; lia | right; left; cbn; lia | right; right; cbn; lia].
+Qed.
+
+Lemma delete_foreground_finalizer_valid :
+  valid_label_name delete_foreground_finalizer.
+Proof.
+  left. split; last done.
+  rewrite /delete_foreground_finalizer /qualified_name_syntax /=.
+  repeat lazymatch goal with | |- _ ∧ _ => split end.
+  all: lazymatch goal with
+       | |- label_extended_character _ => left
+       | |- label_alphanumeric _ => idtac
+       end.
+  all: unfold label_alphanumeric;
+    first [left; cbn; lia | right; left; cbn; lia | right; right; cbn; lia].
+Qed.
+
+Lemma delete_gc_finalizers_distinct :
+  delete_orphan_finalizer ≠ delete_foreground_finalizer.
+Proof. intros Heq. inversion Heq. Qed.
+
+Opaque w8_word_instance.
+
+Lemma delete_finalizers_for_gc_valid m options :
+  valid_finalizers m.(ObjectMetaV.Finalizers') →
+  valid_finalizers (Some (delete_finalizers_for_gc m options)).
+Proof.
+  intros Hvalid.
+  destruct m.(ObjectMetaV.Finalizers') as [old|] eqn:Hold;
+    rewrite /valid_finalizers /= in Hvalid |- *.
+  - rewrite /delete_finalizers_for_gc Hold /= !Forall_app.
+    clear Hold.
+    split; [|split].
+    + induction old as [|finalizer finalizers IH]; first constructor.
+      inversion Hvalid as [|? ? Hname Hnames]; subst.
+      rewrite filter_cons.
+      destruct (decide
+        (finalizer ≠ delete_orphan_finalizer ∧
+         finalizer ≠ delete_foreground_finalizer)); simpl.
+      * constructor; [exact Hname|]. exact (IH Hnames).
+      * exact (IH Hnames).
+    + rewrite /delete_should_orphan_dependents.
+      destruct (delete_gc_policy m options) as [[|]|]; simpl.
+      * constructor; [exact delete_orphan_finalizer_valid|constructor].
+      * constructor.
+      * constructor.
+    + rewrite /delete_should_delete_dependents.
+      destruct (delete_gc_policy m options) as [[|]|]; simpl.
+      * constructor.
+      * constructor; [exact delete_foreground_finalizer_valid|constructor].
+      * constructor.
+  - rewrite /delete_finalizers_for_gc Hold /= !Forall_app.
+    split.
+    + rewrite /delete_should_orphan_dependents.
+      destruct (delete_gc_policy m options) as [[|]|]; simpl.
+      * constructor; [exact delete_orphan_finalizer_valid|constructor].
+      * constructor.
+      * constructor.
+    + rewrite /delete_should_delete_dependents.
+      destruct (delete_gc_policy m options) as [[|]|]; simpl.
+      * constructor.
+      * constructor; [exact delete_foreground_finalizer_valid|constructor].
+      * constructor.
+Qed.
+
+Lemma delete_new_finalizers_valid m options :
+  valid_finalizers m.(ObjectMetaV.Finalizers') →
+  valid_finalizers (delete_new_finalizers m options).
+Proof.
+  intros Hvalid. rewrite /delete_new_finalizers.
+  destruct delete_should_update_finalizers.
+  - by apply delete_finalizers_for_gc_valid.
+  - exact Hvalid.
+Qed.
+
+Lemma delete_finalizer_set_lookup (finalizers : list go_string) finalizer :
+  default false
+    ((list_to_map ((fun finalizer => (finalizer, true)) <$> finalizers) :
+      gmap go_string bool) !! finalizer) =
+  bool_decide (finalizer ∈ finalizers).
+Proof.
+  induction finalizers as [|head finalizers IH].
+  - rewrite fmap_nil list_to_map_nil lookup_empty /=. done.
+  - rewrite fmap_cons list_to_map_cons.
+    destruct (decide (head = finalizer)) as [->|Hneq].
+    + rewrite lookup_insert_eq /=. symmetry.
+      apply bool_decide_eq_true_2. by left.
+    + assert ((<[head := true]>
+          (list_to_map ((fun finalizer => (finalizer, true)) <$> finalizers) :
+            gmap go_string bool)) !! finalizer =
+        (list_to_map ((fun finalizer => (finalizer, true)) <$> finalizers) :
+          gmap go_string bool) !! finalizer) as Hlookup.
+      { apply lookup_insert_ne. exact Hneq. }
+      rewrite Hlookup.
+      simpl. rewrite IH.
+      apply bool_decide_ext. split.
+      * by right.
+      * intros Hmember. apply elem_of_cons in Hmember as [Heq|Hin].
+        -- exfalso. apply Hneq. by symmetry.
+        -- exact Hin.
+Qed.
+
+Lemma wp_shouldOrphanDependents metadata_i metadata_l m options_l options dq :
+  {{{ is_pkg_init apimodel ∗
+      "%Hmetadata" ∷ ⌜ metadata_i = interface.mk (go.PointerType v1.ObjectMeta) #metadata_l ⌝ ∗
+      "Hdeepown_m_l" ∷ ObjectMetaV.deepown_l metadata_l m dq ∗
+      "Hdeepown_options_l" ∷ DeleteOptionsV.deepown_l options_l options dq
+  }}}
+    @! apimodel.shouldOrphanDependents #(interface.ok metadata_i) #options_l
+  {{{ should_orphan, RET #should_orphan;
+      ⌜ should_orphan = delete_should_orphan_dependents m options ⌝ ∗
+      ObjectMetaV.deepown_l metadata_l m dq ∗
+      DeleteOptionsV.deepown_l options_l options dq
+  }}}.
+Proof.
+  wp_start as "H". iNamed "H". subst metadata_i.
+  iDestruct "Hdeepown_options_l" as (options_c) "[Hoptions_l Hoptions]".
+  iDestruct (typed_pointsto_not_null with "Hoptions_l") as %Hoptions_l_not_null.
+  assert (bool_decide (options_l = null) = false) as Hoptions_nonnull_decide.
+  { apply bool_decide_false. done. }
+  iNamed "Hoptions".
+  destruct options.(DeleteOptionsV.OrphanDependents') as [orphan|] eqn:Horphan.
+  - iDestruct "Hdeepown_orphandependents_some" as (orphan_c) "[Horphan_l ->]".
+    iDestruct (typed_pointsto_not_null with "Horphan_l") as %Horphan_l_not_null.
+    assert (bool_decide
+      (v1.DeleteOptions.OrphanDependents' options_c = null) = false)
+      as Horphan_nonnull_decide.
+    { apply bool_decide_false. done. }
+    wp_auto. rewrite Hoptions_nonnull_decide /=. wp_auto.
+    rewrite Horphan_nonnull_decide /=. wp_auto.
+    iAssert (DeleteOptionsV.deepown options_c options dq)
+      with "[Hdeepown_graceperiodseconds_some Hdeepown_preconditions_some
+        Horphan_l Hdeepown_propagationpolicy_some]" as "Hoptions".
+    { rewrite /DeleteOptionsV.deepown Horphan /=. iFrame.
+      iFrame "%"; try (iPureIntro; done). }
+    iApply ("HΦ" $! orphan). iFrame. iPureIntro.
+    rewrite /delete_should_orphan_dependents /delete_gc_policy Horphan /=.
+    by destruct orphan.
+  - assert (v1.DeleteOptions.OrphanDependents' options_c = null) as Horphan_null.
+    { apply (proj2 Hdeepown_orphandependents_none). done. }
+    assert (bool_decide
+      (v1.DeleteOptions.OrphanDependents' options_c = null) = true)
+      as Horphan_null_decide.
+    { apply bool_decide_true. done. }
+    wp_auto. rewrite Hoptions_nonnull_decide /=. wp_auto.
+    rewrite Horphan_null_decide /=. wp_auto.
+    destruct options.(DeleteOptionsV.PropagationPolicy') as [policy|] eqn:Hpolicy.
+    + iDestruct "Hdeepown_propagationpolicy_some" as (policy_c) "[Hpolicy_l ->]".
+      iDestruct (typed_pointsto_not_null with "Hpolicy_l") as %Hpolicy_l_not_null.
+      assert (bool_decide
+        (v1.DeleteOptions.PropagationPolicy' options_c = null) = false)
+        as Hpolicy_nonnull_decide.
+      { apply bool_decide_false. done. }
+      rewrite Hoptions_nonnull_decide /=. wp_auto.
+      rewrite Hpolicy_nonnull_decide /=. wp_auto.
+      iAssert (DeleteOptionsV.deepown options_c options dq)
+        with "[Hdeepown_graceperiodseconds_some Hdeepown_preconditions_some
+          Hpolicy_l]" as "Hoptions".
+      { rewrite /DeleteOptionsV.deepown Horphan Hpolicy /=. iFrame.
+        iFrame "%"; try (iPureIntro; done). }
+      wp_if_destruct.
+      * iApply ("HΦ" $! true). iFrame. iPureIntro.
+        rewrite /delete_should_orphan_dependents /delete_gc_policy Horphan Hpolicy /=.
+        repeat case_decide; done.
+      * wp_if_destruct.
+        -- iApply ("HΦ" $! false). iFrame. iPureIntro.
+           rewrite /delete_should_orphan_dependents /delete_gc_policy Horphan Hpolicy /=.
+           repeat case_decide; done.
+        -- wp_if_destruct.
+           { iApply ("HΦ" $! false). iFrame. iPureIntro.
+             rewrite /delete_should_orphan_dependents /delete_gc_policy
+               Horphan Hpolicy /=.
+             repeat case_decide; done. }
+           { assert (delete_should_orphan_dependents m options =
+              match delete_existing_gc_policy
+                (default [] m.(ObjectMetaV.Finalizers')) with
+              | Some true => true
+              | _ => false
+             end) as Hshould_fallback.
+           { rewrite /delete_should_orphan_dependents /delete_gc_policy
+               Horphan Hpolicy /=.
+             repeat case_decide; try congruence; done. }
+           iDestruct "Hdeepown_m_l" as (metadata_c) "[Hmetadata_l Hmetadata]".
+           wp_bind.
+           wp_apply (v1.wp_GetFinalizers metadata_l metadata_c dq
+             with "[$Hmetadata_l]") as "Hmetadata_l".
+           set (sl := metadata_c.(v1.ObjectMeta.Finalizers')).
+           iNamed "Hmetadata".
+           destruct m.(ObjectMetaV.Finalizers') as [finalizers|] eqn:Hfinalizers.
+           ++ iDestruct "Hdeepown_finalizers_some" as (cfinalizers) "[Hsl ->]".
+              iAssert ((sl ↦*{dq} finalizers -∗
+                ObjectMetaV.deepown_l metadata_l m dq)%I)
+                with "[Hmetadata_l Hdeepown_creationtimestamp
+                  Hdeepown_deletiontimestamp_some
+                  Hdeepown_deletiongraceperiodseconds_some Hdeepown_labels_some
+                  Hdeepown_annotations_some Hdeepown_ownerreferences_some
+                  Hdeepown_managedfields_some]" as "Hrestore_m".
+              { iIntros "Hsl". iExists metadata_c. iFrame.
+                rewrite /ObjectMetaV.deepown Hfinalizers /=. iFrame.
+                iFrame "%"; try (iPureIntro; done). }
+              iDestruct (own_slice_len with "Hsl") as %[Hsl_len _].
+              iDestruct (own_slice_wf with "Hsl") as %Hsl_wf.
+              set I := (∃ (i : w64) (f : go_string),
+                "Hi" ∷ i_ptr ↦ i ∗
+                "Hf" ∷ f_ptr ↦ f ∗
+                "Hsl" ∷ sl ↦*{dq} finalizers ∗
+                "%Hi_bounds" ∷ ⌜ 0 ≤ sint.Z i ≤ sint.Z sl.(slice.len) ⌝ ∗
+                "%Hscan" ∷ ⌜ delete_existing_gc_policy
+                  (drop (sint.nat i) finalizers) =
+                  delete_existing_gc_policy finalizers ⌝)%I.
+              iAssert I with "[i f Hsl]" as "Hloop".
+              { iExists (W64 0), (zero_val go_string). iFrame.
+                iPureIntro. split; [word|done]. }
+              wp_for "Hloop". wp_if_destruct.
+              ** destruct (decide (0 ≤ sint.Z i < sint.Z sl.(slice.len)))
+                   as [_|Hbounds]; last word.
+                 destruct (lookup_lt_is_Some_2 finalizers (sint.nat i))
+                   as [current Hcurrent_lookup].
+                 { rewrite Hsl_len. word. }
+                 wp_apply (wp_load_slice_index with "[$Hsl]"); [word|done|].
+                 iIntros "Hsl". wp_auto.
+                 assert (drop (sint.nat i) finalizers =
+                   current :: drop (S (sint.nat i)) finalizers) as Hdrop.
+                 { apply drop_S. exact Hcurrent_lookup. }
+                 wp_if_destruct.
+                 --- iApply wp_for_post_return.
+                     rewrite return_val_unseal /return_val_def.
+                     rewrite exception_do_unseal /exception_do_def. wp_auto.
+                     rewrite exception_seq_unseal /exception.exception_seq_def. wp_auto.
+                     iPoseProof ("Hrestore_m" with "Hsl") as "Hdeepown_m_l".
+                     iApply ("HΦ" $! true). iFrame. iPureIntro.
+                     rewrite Hdrop /= in Hscan.
+                     rewrite Hshould_fallback /= -Hscan. done.
+                 --- wp_if_destruct.
+                     +++ iApply wp_for_post_return.
+                         rewrite return_val_unseal /return_val_def.
+                         rewrite exception_do_unseal /exception_do_def. wp_auto.
+                         rewrite exception_seq_unseal /exception.exception_seq_def. wp_auto.
+                         iPoseProof ("Hrestore_m" with "Hsl") as "Hdeepown_m_l".
+                         iApply ("HΦ" $! false). iFrame. iPureIntro.
+                         rewrite Hshould_fallback /=.
+                         rewrite Hdrop /= in Hscan.
+                         rewrite -Hscan.
+                         done.
+                     +++ iApply wp_for_post_do. wp_auto.
+                         iAssert I with "[Hi Hf Hsl]" as "Hloop".
+                         { iExists (word.add i (W64 1)), current. iFrame.
+                           iPureIntro. split; [word|].
+                           assert (current ≠ delete_orphan_finalizer) as Hnot_orphan.
+                           { rewrite /delete_orphan_finalizer. congruence. }
+                           assert (current ≠ delete_foreground_finalizer) as Hnot_foreground.
+                           { rewrite /delete_foreground_finalizer. congruence. }
+                           rewrite Hdrop /= in Hscan.
+                           repeat case_decide; try contradiction.
+                           assert (sint.nat (word.add i (W64 1)) =
+                             S (sint.nat i)) as -> by word.
+                           exact Hscan. }
+                         iFrame.
+              ** assert (sint.nat i = length finalizers) as Hi_end.
+                 { rewrite Hsl_len. word. }
+                 rewrite Hi_end drop_all in Hscan.
+                 iPoseProof ("Hrestore_m" with "Hsl") as "Hdeepown_m_l".
+                 iApply ("HΦ" $! false). iFrame. iPureIntro.
+                 rewrite Hshould_fallback /= -Hscan. done.
+           ++ assert (sl = slice.nil) as ->.
+              { apply (proj2 Hdeepown_finalizers_none). done. }
+              iAssert (ObjectMetaV.deepown_l metadata_l m dq)
+                with "[Hmetadata_l Hdeepown_creationtimestamp
+                  Hdeepown_deletiontimestamp_some
+                  Hdeepown_deletiongraceperiodseconds_some Hdeepown_labels_some
+                  Hdeepown_annotations_some Hdeepown_ownerreferences_some
+                  Hdeepown_managedfields_some]" as "Hdeepown_m_l".
+              { iExists metadata_c. iFrame.
+                rewrite /ObjectMetaV.deepown Hfinalizers /=. iFrame.
+                iFrame "%"; try (iPureIntro; done). }
+              set I_nil := ("Hi" ∷ i_ptr ↦ (W64 0) ∗
+                "Hf" ∷ f_ptr ↦ (zero_val go_string))%I.
+              iAssert I_nil with "[i f]" as "Hloop"; first iFrame.
+              wp_for "Hloop". wp_if_destruct; first word.
+              iApply ("HΦ" $! false). iFrame. iPureIntro.
+              rewrite Hshould_fallback /=. done. }
+    + assert (v1.DeleteOptions.PropagationPolicy' options_c = null) as Hpolicy_null.
+      { apply (proj2 Hdeepown_propagationpolicy_none). done. }
+      assert (bool_decide
+        (v1.DeleteOptions.PropagationPolicy' options_c = null) = true)
+        as Hpolicy_null_decide.
+      { apply bool_decide_true. done. }
+      rewrite Hoptions_nonnull_decide /=. wp_auto.
+      rewrite Hpolicy_null_decide /=. wp_auto.
+      iAssert (DeleteOptionsV.deepown options_c options dq)
+        with "[Hdeepown_graceperiodseconds_some Hdeepown_preconditions_some]"
+        as "Hoptions".
+      { rewrite /DeleteOptionsV.deepown Horphan Hpolicy /=. iFrame.
+        iFrame "%"; try (iPureIntro; done). }
+      assert (delete_should_orphan_dependents m options =
+        match delete_existing_gc_policy
+          (default [] m.(ObjectMetaV.Finalizers')) with
+        | Some true => true
+        | _ => false
+        end) as Hshould_fallback.
+      { rewrite /delete_should_orphan_dependents /delete_gc_policy
+          Horphan Hpolicy /=. done. }
+      iDestruct "Hdeepown_m_l" as (metadata_c) "[Hmetadata_l Hmetadata]".
+      wp_bind.
+      wp_apply (v1.wp_GetFinalizers metadata_l metadata_c dq
+        with "[$Hmetadata_l]") as "Hmetadata_l".
+      set (sl := metadata_c.(v1.ObjectMeta.Finalizers')).
+      iNamed "Hmetadata".
+      destruct m.(ObjectMetaV.Finalizers') as [finalizers|] eqn:Hfinalizers.
+      * iDestruct "Hdeepown_finalizers_some" as (cfinalizers) "[Hsl ->]".
+        iAssert ((sl ↦*{dq} finalizers -∗
+          ObjectMetaV.deepown_l metadata_l m dq)%I)
+          with "[Hmetadata_l Hdeepown_creationtimestamp
+            Hdeepown_deletiontimestamp_some
+            Hdeepown_deletiongraceperiodseconds_some Hdeepown_labels_some
+            Hdeepown_annotations_some Hdeepown_ownerreferences_some
+            Hdeepown_managedfields_some]" as "Hrestore_m".
+        { iIntros "Hsl". iExists metadata_c. iFrame.
+          rewrite /ObjectMetaV.deepown Hfinalizers /=. iFrame.
+          iFrame "%"; try (iPureIntro; done). }
+        iDestruct (own_slice_len with "Hsl") as %[Hsl_len _].
+        iDestruct (own_slice_wf with "Hsl") as %Hsl_wf.
+        set I := (∃ (i : w64) (f : go_string),
+          "Hi" ∷ i_ptr ↦ i ∗
+          "Hf" ∷ f_ptr ↦ f ∗
+          "Hsl" ∷ sl ↦*{dq} finalizers ∗
+          "%Hi_bounds" ∷ ⌜ 0 ≤ sint.Z i ≤ sint.Z sl.(slice.len) ⌝ ∗
+          "%Hscan" ∷ ⌜ delete_existing_gc_policy
+            (drop (sint.nat i) finalizers) =
+            delete_existing_gc_policy finalizers ⌝)%I.
+        iAssert I with "[i f Hsl]" as "Hloop".
+        { iExists (W64 0), (zero_val go_string). iFrame.
+          iPureIntro. split; [word|done]. }
+        wp_for "Hloop". wp_if_destruct.
+        -- destruct (decide (0 ≤ sint.Z i < sint.Z sl.(slice.len)))
+             as [_|Hbounds]; last word.
+           destruct (lookup_lt_is_Some_2 finalizers (sint.nat i))
+             as [current Hcurrent_lookup].
+           { rewrite Hsl_len. word. }
+           wp_apply (wp_load_slice_index with "[$Hsl]"); [word|done|].
+           iIntros "Hsl". wp_auto.
+           assert (drop (sint.nat i) finalizers =
+             current :: drop (S (sint.nat i)) finalizers) as Hdrop.
+           { apply drop_S. exact Hcurrent_lookup. }
+           wp_if_destruct.
+           ++ iApply wp_for_post_return.
+              rewrite return_val_unseal /return_val_def.
+              rewrite exception_do_unseal /exception_do_def. wp_auto.
+              rewrite exception_seq_unseal /exception.exception_seq_def. wp_auto.
+              iPoseProof ("Hrestore_m" with "Hsl") as "Hdeepown_m_l".
+              iApply ("HΦ" $! true). iFrame. iPureIntro.
+              rewrite Hshould_fallback /=.
+              rewrite Hdrop /= in Hscan.
+              rewrite -Hscan.
+              done.
+           ++ wp_if_destruct.
+              ** iApply wp_for_post_return.
+                 rewrite return_val_unseal /return_val_def.
+                 rewrite exception_do_unseal /exception_do_def. wp_auto.
+                 rewrite exception_seq_unseal /exception.exception_seq_def. wp_auto.
+                 iPoseProof ("Hrestore_m" with "Hsl") as "Hdeepown_m_l".
+                 iApply ("HΦ" $! false). iFrame. iPureIntro.
+                 rewrite Hshould_fallback /=.
+                 rewrite Hdrop /= in Hscan.
+                 rewrite -Hscan.
+                 done.
+              ** iApply wp_for_post_do. wp_auto.
+                 iAssert I with "[Hi Hf Hsl]" as "Hloop".
+                 { iExists (word.add i (W64 1)), current. iFrame.
+                   iPureIntro. split; [word|].
+                   assert (current ≠ delete_orphan_finalizer) as Hnot_orphan.
+                   { rewrite /delete_orphan_finalizer. congruence. }
+                   assert (current ≠ delete_foreground_finalizer) as Hnot_foreground.
+                   { rewrite /delete_foreground_finalizer. congruence. }
+                   rewrite Hdrop /= in Hscan.
+                   repeat case_decide; try contradiction.
+                   assert (sint.nat (word.add i (W64 1)) =
+                     S (sint.nat i)) as -> by word.
+                   exact Hscan. }
+                 iFrame.
+        -- assert (sint.nat i = length finalizers) as Hi_end.
+           { rewrite Hsl_len. word. }
+           rewrite Hi_end drop_all in Hscan.
+           iPoseProof ("Hrestore_m" with "Hsl") as "Hdeepown_m_l".
+           iApply ("HΦ" $! false). iFrame. iPureIntro.
+           rewrite Hshould_fallback /= -Hscan. done.
+      * assert (sl = slice.nil) as ->.
+        { apply (proj2 Hdeepown_finalizers_none). done. }
+        iAssert (ObjectMetaV.deepown_l metadata_l m dq)
+          with "[Hmetadata_l Hdeepown_creationtimestamp
+            Hdeepown_deletiontimestamp_some
+            Hdeepown_deletiongraceperiodseconds_some Hdeepown_labels_some
+            Hdeepown_annotations_some Hdeepown_ownerreferences_some
+            Hdeepown_managedfields_some]" as "Hdeepown_m_l".
+        { iExists metadata_c. iFrame.
+          rewrite /ObjectMetaV.deepown Hfinalizers /=. iFrame.
+          iFrame "%"; try (iPureIntro; done). }
+        set I_nil := ("Hi" ∷ i_ptr ↦ (W64 0) ∗
+          "Hf" ∷ f_ptr ↦ (zero_val go_string))%I.
+        iAssert I_nil with "[i f]" as "Hloop"; first iFrame.
+        wp_for "Hloop". wp_if_destruct; first word.
+        iApply ("HΦ" $! false). iFrame. iPureIntro.
+        rewrite Hshould_fallback /=. done.
+Qed.
+
+Lemma wp_shouldDeleteDependents metadata_i metadata_l m options_l options dq :
+  {{{ is_pkg_init apimodel ∗
+      "%Hmetadata" ∷ ⌜ metadata_i = interface.mk (go.PointerType v1.ObjectMeta) #metadata_l ⌝ ∗
+      "Hdeepown_m_l" ∷ ObjectMetaV.deepown_l metadata_l m dq ∗
+      "Hdeepown_options_l" ∷ DeleteOptionsV.deepown_l options_l options dq
+  }}}
+    @! apimodel.shouldDeleteDependents #(interface.ok metadata_i) #options_l
+  {{{ should_delete, RET #should_delete;
+      ⌜ should_delete = delete_should_delete_dependents m options ⌝ ∗
+      ObjectMetaV.deepown_l metadata_l m dq ∗
+      DeleteOptionsV.deepown_l options_l options dq
+  }}}.
+Proof.
+  wp_start as "H". iNamed "H". subst metadata_i.
+  iDestruct "Hdeepown_options_l" as (options_c) "[Hoptions_l Hoptions]".
+  iDestruct (typed_pointsto_not_null with "Hoptions_l") as %Hoptions_l_not_null.
+  assert (bool_decide (options_l = null) = false) as Hoptions_nonnull_decide.
+  { apply bool_decide_false. done. }
+  iNamed "Hoptions".
+  destruct options.(DeleteOptionsV.OrphanDependents') as [orphan|] eqn:Horphan.
+  - iDestruct "Hdeepown_orphandependents_some" as (orphan_c) "[Horphan_l ->]".
+    iDestruct (typed_pointsto_not_null with "Horphan_l") as %Horphan_l_not_null.
+    assert (bool_decide
+      (v1.DeleteOptions.OrphanDependents' options_c = null) = false)
+      as Horphan_nonnull_decide.
+    { apply bool_decide_false. done. }
+    wp_auto. rewrite Hoptions_nonnull_decide /=. wp_auto.
+    rewrite Horphan_nonnull_decide /=. wp_auto.
+    iAssert (DeleteOptionsV.deepown options_c options dq)
+      with "[Hdeepown_graceperiodseconds_some Hdeepown_preconditions_some
+        Horphan_l Hdeepown_propagationpolicy_some]" as "Hoptions".
+    { rewrite /DeleteOptionsV.deepown Horphan /=. iFrame.
+      iFrame "%"; try (iPureIntro; done). }
+    iApply ("HΦ" $! false). iFrame. iPureIntro.
+    rewrite /delete_should_delete_dependents /delete_gc_policy Horphan /=.
+    by destruct orphan.
+  - assert (v1.DeleteOptions.OrphanDependents' options_c = null) as Horphan_null.
+    { apply (proj2 Hdeepown_orphandependents_none). done. }
+    assert (bool_decide
+      (v1.DeleteOptions.OrphanDependents' options_c = null) = true)
+      as Horphan_null_decide.
+    { apply bool_decide_true. done. }
+    wp_auto. rewrite Hoptions_nonnull_decide /=. wp_auto.
+    rewrite Horphan_null_decide /=. wp_auto.
+    destruct options.(DeleteOptionsV.PropagationPolicy') as [policy|] eqn:Hpolicy.
+    + iDestruct "Hdeepown_propagationpolicy_some" as (policy_c) "[Hpolicy_l ->]".
+      iDestruct (typed_pointsto_not_null with "Hpolicy_l") as %Hpolicy_l_not_null.
+      assert (bool_decide
+        (v1.DeleteOptions.PropagationPolicy' options_c = null) = false)
+        as Hpolicy_nonnull_decide.
+      { apply bool_decide_false. done. }
+      rewrite Hoptions_nonnull_decide /=. wp_auto.
+      rewrite Hpolicy_nonnull_decide /=. wp_auto.
+      iAssert (DeleteOptionsV.deepown options_c options dq)
+        with "[Hdeepown_graceperiodseconds_some Hdeepown_preconditions_some
+          Hpolicy_l]" as "Hoptions".
+      { rewrite /DeleteOptionsV.deepown Horphan Hpolicy /=. iFrame.
+        iFrame "%"; try (iPureIntro; done). }
+      wp_if_destruct.
+      * iApply ("HΦ" $! true). iFrame. iPureIntro.
+        rewrite /delete_should_delete_dependents /delete_gc_policy Horphan Hpolicy /=.
+        repeat case_decide; done.
+      * wp_if_destruct.
+        -- iApply ("HΦ" $! false). iFrame. iPureIntro.
+           rewrite /delete_should_delete_dependents /delete_gc_policy Horphan Hpolicy /=.
+           repeat case_decide; done.
+        -- wp_if_destruct.
+           { iApply ("HΦ" $! false). iFrame. iPureIntro.
+             rewrite /delete_should_delete_dependents /delete_gc_policy
+               Horphan Hpolicy /=.
+             repeat case_decide; done. }
+           { assert (delete_should_delete_dependents m options =
+              match delete_existing_gc_policy
+                (default [] m.(ObjectMetaV.Finalizers')) with
+              | Some false => true
+              | _ => false
+             end) as Hshould_fallback.
+           { rewrite /delete_should_delete_dependents /delete_gc_policy
+               Horphan Hpolicy /=.
+             repeat case_decide; try congruence; done. }
+           iDestruct "Hdeepown_m_l" as (metadata_c) "[Hmetadata_l Hmetadata]".
+           wp_bind.
+           wp_apply (v1.wp_GetFinalizers metadata_l metadata_c dq
+             with "[$Hmetadata_l]") as "Hmetadata_l".
+           set (sl := metadata_c.(v1.ObjectMeta.Finalizers')).
+           iNamed "Hmetadata".
+           destruct m.(ObjectMetaV.Finalizers') as [finalizers|] eqn:Hfinalizers.
+           ++ iDestruct "Hdeepown_finalizers_some" as (cfinalizers) "[Hsl ->]".
+              iAssert ((sl ↦*{dq} finalizers -∗
+                ObjectMetaV.deepown_l metadata_l m dq)%I)
+                with "[Hmetadata_l Hdeepown_creationtimestamp
+                  Hdeepown_deletiontimestamp_some
+                  Hdeepown_deletiongraceperiodseconds_some Hdeepown_labels_some
+                  Hdeepown_annotations_some Hdeepown_ownerreferences_some
+                  Hdeepown_managedfields_some]" as "Hrestore_m".
+              { iIntros "Hsl". iExists metadata_c. iFrame.
+                rewrite /ObjectMetaV.deepown Hfinalizers /=. iFrame.
+                iFrame "%"; try (iPureIntro; done). }
+              iDestruct (own_slice_len with "Hsl") as %[Hsl_len _].
+              iDestruct (own_slice_wf with "Hsl") as %Hsl_wf.
+              set I := (∃ (i : w64) (f : go_string),
+                "Hi" ∷ i_ptr ↦ i ∗
+                "Hf" ∷ f_ptr ↦ f ∗
+                "Hsl" ∷ sl ↦*{dq} finalizers ∗
+                "%Hi_bounds" ∷ ⌜ 0 ≤ sint.Z i ≤ sint.Z sl.(slice.len) ⌝ ∗
+                "%Hscan" ∷ ⌜ delete_existing_gc_policy
+                  (drop (sint.nat i) finalizers) =
+                  delete_existing_gc_policy finalizers ⌝)%I.
+              iAssert I with "[i f Hsl]" as "Hloop".
+              { iExists (W64 0), (zero_val go_string). iFrame.
+                iPureIntro. split; [word|done]. }
+              wp_for "Hloop". wp_if_destruct.
+              ** destruct (decide (0 ≤ sint.Z i < sint.Z sl.(slice.len)))
+                   as [_|Hbounds]; last word.
+                 destruct (lookup_lt_is_Some_2 finalizers (sint.nat i))
+                   as [current Hcurrent_lookup].
+                 { rewrite Hsl_len. word. }
+                 wp_apply (wp_load_slice_index with "[$Hsl]"); [word|done|].
+                 iIntros "Hsl". wp_auto.
+                 assert (drop (sint.nat i) finalizers =
+                   current :: drop (S (sint.nat i)) finalizers) as Hdrop.
+                 { apply drop_S. exact Hcurrent_lookup. }
+                 wp_if_destruct.
+                 --- iApply wp_for_post_return.
+                     rewrite return_val_unseal /return_val_def.
+                     rewrite exception_do_unseal /exception_do_def. wp_auto.
+                     rewrite exception_seq_unseal /exception.exception_seq_def. wp_auto.
+                     iPoseProof ("Hrestore_m" with "Hsl") as "Hdeepown_m_l".
+                     iApply ("HΦ" $! true). iFrame. iPureIntro.
+                     rewrite Hshould_fallback /=.
+                     rewrite Hdrop /= in Hscan.
+                     rewrite -Hscan.
+                     done.
+                 --- wp_if_destruct.
+                     +++ iApply wp_for_post_return.
+                         rewrite return_val_unseal /return_val_def.
+                         rewrite exception_do_unseal /exception_do_def. wp_auto.
+                         rewrite exception_seq_unseal /exception.exception_seq_def. wp_auto.
+                         iPoseProof ("Hrestore_m" with "Hsl") as "Hdeepown_m_l".
+                         iApply ("HΦ" $! false). iFrame. iPureIntro.
+                         rewrite Hshould_fallback /=.
+                         rewrite Hdrop /= in Hscan.
+                         rewrite -Hscan.
+                         done.
+                     +++ iApply wp_for_post_do. wp_auto.
+                         iAssert I with "[Hi Hf Hsl]" as "Hloop".
+                         { iExists (word.add i (W64 1)), current. iFrame.
+                           iPureIntro. split; [word|].
+                           assert (current ≠ delete_orphan_finalizer) as Hnot_orphan.
+                           { rewrite /delete_orphan_finalizer. congruence. }
+                           assert (current ≠ delete_foreground_finalizer) as Hnot_foreground.
+                           { rewrite /delete_foreground_finalizer. congruence. }
+                           rewrite Hdrop /= in Hscan.
+                           repeat case_decide; try contradiction.
+                           assert (sint.nat (word.add i (W64 1)) =
+                             S (sint.nat i)) as -> by word.
+                           exact Hscan. }
+                         iFrame.
+              ** assert (sint.nat i = length finalizers) as Hi_end.
+                 { rewrite Hsl_len. word. }
+                 rewrite Hi_end drop_all in Hscan.
+                 iPoseProof ("Hrestore_m" with "Hsl") as "Hdeepown_m_l".
+                 iApply ("HΦ" $! false). iFrame. iPureIntro.
+                 rewrite Hshould_fallback /= -Hscan. done.
+           ++ assert (sl = slice.nil) as ->.
+              { apply (proj2 Hdeepown_finalizers_none). done. }
+              iAssert (ObjectMetaV.deepown_l metadata_l m dq)
+                with "[Hmetadata_l Hdeepown_creationtimestamp
+                  Hdeepown_deletiontimestamp_some
+                  Hdeepown_deletiongraceperiodseconds_some Hdeepown_labels_some
+                  Hdeepown_annotations_some Hdeepown_ownerreferences_some
+                  Hdeepown_managedfields_some]" as "Hdeepown_m_l".
+              { iExists metadata_c. iFrame.
+                rewrite /ObjectMetaV.deepown Hfinalizers /=. iFrame.
+                iFrame "%"; try (iPureIntro; done). }
+              set I_nil := ("Hi" ∷ i_ptr ↦ (W64 0) ∗
+                "Hf" ∷ f_ptr ↦ (zero_val go_string))%I.
+              iAssert I_nil with "[i f]" as "Hloop"; first iFrame.
+              wp_for "Hloop". wp_if_destruct; first word.
+              iApply ("HΦ" $! false). iFrame. iPureIntro.
+              rewrite Hshould_fallback /=. done. }
+    + assert (v1.DeleteOptions.PropagationPolicy' options_c = null) as Hpolicy_null.
+      { apply (proj2 Hdeepown_propagationpolicy_none). done. }
+      assert (bool_decide
+        (v1.DeleteOptions.PropagationPolicy' options_c = null) = true)
+        as Hpolicy_null_decide.
+      { apply bool_decide_true. done. }
+      rewrite Hoptions_nonnull_decide /=. wp_auto.
+      rewrite Hpolicy_null_decide /=. wp_auto.
+      iAssert (DeleteOptionsV.deepown options_c options dq)
+        with "[Hdeepown_graceperiodseconds_some Hdeepown_preconditions_some]"
+        as "Hoptions".
+      { rewrite /DeleteOptionsV.deepown Horphan Hpolicy /=. iFrame.
+        iFrame "%"; try (iPureIntro; done). }
+      assert (delete_should_delete_dependents m options =
+        match delete_existing_gc_policy
+          (default [] m.(ObjectMetaV.Finalizers')) with
+        | Some false => true
+        | _ => false
+        end) as Hshould_fallback.
+      { rewrite /delete_should_delete_dependents /delete_gc_policy
+          Horphan Hpolicy /=. done. }
+      iDestruct "Hdeepown_m_l" as (metadata_c) "[Hmetadata_l Hmetadata]".
+      wp_bind.
+      wp_apply (v1.wp_GetFinalizers metadata_l metadata_c dq
+        with "[$Hmetadata_l]") as "Hmetadata_l".
+      set (sl := metadata_c.(v1.ObjectMeta.Finalizers')).
+      iNamed "Hmetadata".
+      destruct m.(ObjectMetaV.Finalizers') as [finalizers|] eqn:Hfinalizers.
+      * iDestruct "Hdeepown_finalizers_some" as (cfinalizers) "[Hsl ->]".
+        iAssert ((sl ↦*{dq} finalizers -∗
+          ObjectMetaV.deepown_l metadata_l m dq)%I)
+          with "[Hmetadata_l Hdeepown_creationtimestamp
+            Hdeepown_deletiontimestamp_some
+            Hdeepown_deletiongraceperiodseconds_some Hdeepown_labels_some
+            Hdeepown_annotations_some Hdeepown_ownerreferences_some
+            Hdeepown_managedfields_some]" as "Hrestore_m".
+        { iIntros "Hsl". iExists metadata_c. iFrame.
+          rewrite /ObjectMetaV.deepown Hfinalizers /=. iFrame.
+          iFrame "%"; try (iPureIntro; done). }
+        iDestruct (own_slice_len with "Hsl") as %[Hsl_len _].
+        iDestruct (own_slice_wf with "Hsl") as %Hsl_wf.
+        set I := (∃ (i : w64) (f : go_string),
+          "Hi" ∷ i_ptr ↦ i ∗
+          "Hf" ∷ f_ptr ↦ f ∗
+          "Hsl" ∷ sl ↦*{dq} finalizers ∗
+          "%Hi_bounds" ∷ ⌜ 0 ≤ sint.Z i ≤ sint.Z sl.(slice.len) ⌝ ∗
+          "%Hscan" ∷ ⌜ delete_existing_gc_policy
+            (drop (sint.nat i) finalizers) =
+            delete_existing_gc_policy finalizers ⌝)%I.
+        iAssert I with "[i f Hsl]" as "Hloop".
+        { iExists (W64 0), (zero_val go_string). iFrame.
+          iPureIntro. split; [word|done]. }
+        wp_for "Hloop". wp_if_destruct.
+        -- destruct (decide (0 ≤ sint.Z i < sint.Z sl.(slice.len)))
+             as [_|Hbounds]; last word.
+           destruct (lookup_lt_is_Some_2 finalizers (sint.nat i))
+             as [current Hcurrent_lookup].
+           { rewrite Hsl_len. word. }
+           wp_apply (wp_load_slice_index with "[$Hsl]"); [word|done|].
+           iIntros "Hsl". wp_auto.
+           assert (drop (sint.nat i) finalizers =
+             current :: drop (S (sint.nat i)) finalizers) as Hdrop.
+           { apply drop_S. exact Hcurrent_lookup. }
+           wp_if_destruct.
+           ++ iApply wp_for_post_return.
+              rewrite return_val_unseal /return_val_def.
+              rewrite exception_do_unseal /exception_do_def. wp_auto.
+              rewrite exception_seq_unseal /exception.exception_seq_def. wp_auto.
+              iPoseProof ("Hrestore_m" with "Hsl") as "Hdeepown_m_l".
+              iApply ("HΦ" $! true). iFrame. iPureIntro.
+              rewrite Hshould_fallback /=.
+              rewrite Hdrop /= in Hscan.
+              rewrite -Hscan.
+              done.
+           ++ wp_if_destruct.
+              ** iApply wp_for_post_return.
+                 rewrite return_val_unseal /return_val_def.
+                 rewrite exception_do_unseal /exception_do_def. wp_auto.
+                 rewrite exception_seq_unseal /exception.exception_seq_def. wp_auto.
+                 iPoseProof ("Hrestore_m" with "Hsl") as "Hdeepown_m_l".
+                 iApply ("HΦ" $! false). iFrame. iPureIntro.
+                 rewrite Hshould_fallback /=.
+                 rewrite Hdrop /= in Hscan.
+                 rewrite -Hscan.
+                 done.
+              ** iApply wp_for_post_do. wp_auto.
+                 iAssert I with "[Hi Hf Hsl]" as "Hloop".
+                 { iExists (word.add i (W64 1)), current. iFrame.
+                   iPureIntro. split; [word|].
+                   assert (current ≠ delete_orphan_finalizer) as Hnot_orphan.
+                   { rewrite /delete_orphan_finalizer. congruence. }
+                   assert (current ≠ delete_foreground_finalizer) as Hnot_foreground.
+                   { rewrite /delete_foreground_finalizer. congruence. }
+                   rewrite Hdrop /= in Hscan.
+                   repeat case_decide; try contradiction.
+                   assert (sint.nat (word.add i (W64 1)) =
+                     S (sint.nat i)) as -> by word.
+                   exact Hscan. }
+                 iFrame.
+        -- assert (sint.nat i = length finalizers) as Hi_end.
+           { rewrite Hsl_len. word. }
+           rewrite Hi_end drop_all in Hscan.
+           iPoseProof ("Hrestore_m" with "Hsl") as "Hdeepown_m_l".
+           iApply ("HΦ" $! false). iFrame. iPureIntro.
+           rewrite Hshould_fallback /= -Hscan. done.
+      * assert (sl = slice.nil) as ->.
+        { apply (proj2 Hdeepown_finalizers_none). done. }
+        iAssert (ObjectMetaV.deepown_l metadata_l m dq)
+          with "[Hmetadata_l Hdeepown_creationtimestamp
+            Hdeepown_deletiontimestamp_some
+            Hdeepown_deletiongraceperiodseconds_some Hdeepown_labels_some
+            Hdeepown_annotations_some Hdeepown_ownerreferences_some
+            Hdeepown_managedfields_some]" as "Hdeepown_m_l".
+        { iExists metadata_c. iFrame.
+          rewrite /ObjectMetaV.deepown Hfinalizers /=. iFrame.
+          iFrame "%"; try (iPureIntro; done). }
+        set I_nil := ("Hi" ∷ i_ptr ↦ (W64 0) ∗
+          "Hf" ∷ f_ptr ↦ (zero_val go_string))%I.
+        iAssert I_nil with "[i f]" as "Hloop"; first iFrame.
+        wp_for "Hloop". wp_if_destruct; first word.
+        iApply ("HΦ" $! false). iFrame. iPureIntro.
+        rewrite Hshould_fallback /=. done.
+Qed.
+
+Lemma wp_slice_literal_non_nil `[!ZeroVal V] `[!TypedPointsto V]
+    `[!IntoValTyped V t]
+    `{!st ↓u (go.SliceType t)} (l : list V) kvs Φ :
+  let len := go.array_literal_size kvs in
+  WP (CompositeLiteral (go.ArrayType len t) (LiteralValueV kvs))
+    {{ v,
+      ⌜ v = #(array.mk len l) ⌝ ∗
+      (∀ sl_ptr,
+        let sl := slice.mk sl_ptr (W64 len) (W64 len) in
+        (sl ↦* l ∗ own_slice_cap V sl 1 ∗ ⌜ sl ≠ slice.nil ⌝) -∗
+        Φ #sl) }}
+  -∗
+  WP (CompositeLiteral st (LiteralValueV kvs)) {{ Φ }}.
+Proof.
+  iIntros "* HΦ".
+  pose proof go.composite_literal_slice.
+  wp_pures. destruct decide; last by iApply wp_AngelicExit.
+  wp_pures. wp_alloc_auto.
+  iDestruct (typed_pointsto_not_null with "tmp") as %Hnotnull.
+  wp_pure. wp_pure.
+  wp_apply (wp_wand with "HΦ"). iIntros "% [-> HΦ]". wp_auto.
+  rewrite decide_True.
+  1: { enough (0 ≤ go.array_literal_size kvs) by word.
+    unfold go.array_literal_size. destruct foldl. lia. }
+  wp_auto. iDestruct (array_len with "tmp") as %Hlen.
+  rewrite !go.array_index_ref_0 /=.
+  wp_end.
+  - iDestruct (slice_array with "tmp") as "$".
+    { simpl. word. }
+    iSplitL.
+    + iApply own_slice_cap_empty; simpl; [done|word].
+    + iPureIntro. intros Hnil. apply Hnotnull.
+      by inversion Hnil.
+  - ereplace (word.sub ?[a] ?[b]) with (?a) by word. done.
+Qed.
+
+Lemma wp_deletionFinalizersForGarbageCollection metadata_i metadata_l m options_l options dq :
+  {{{ is_pkg_init apimodel ∗
+      "%Hmetadata" ∷ ⌜ metadata_i = interface.mk (go.PointerType v1.ObjectMeta) #metadata_l ⌝ ∗
+      "Hdeepown_m_l" ∷ ObjectMetaV.deepown_l metadata_l m dq ∗
+      "Hdeepown_options_l" ∷ DeleteOptionsV.deepown_l options_l options dq ∗
+      "%Hvalid_finalizers" ∷ ⌜ valid_finalizers m.(ObjectMetaV.Finalizers') ⌝
+  }}}
+    @! apimodel.deletionFinalizersForGarbageCollection #(interface.ok metadata_i) #options_l
+  {{{ should_update_finalizers new_finalizers_sl new_finalizers, RET (#should_update_finalizers, #new_finalizers_sl);
+      ⌜ should_update_finalizers = delete_should_update_finalizers m options ⌝ ∗
+      ⌜ new_finalizers = delete_new_finalizers m options ⌝ ∗
+      ⌜ valid_finalizers new_finalizers ⌝ ∗
+      ⌜ new_finalizers_sl = slice.nil ↔ new_finalizers = None ⌝ ∗
+      (if should_update_finalizers then
+        match new_finalizers with
+        | Some fs => ∃ cfs, new_finalizers_sl ↦* cfs ∗ ⌜ cfs = fs ⌝
+        | None => True%I
+        end
+      else True%I) ∗
+      ObjectMetaV.deepown_l metadata_l m dq ∗
+      DeleteOptionsV.deepown_l options_l options dq
+  }}}.
+Proof.
+  wp_start as "H". iNamed "H". subst metadata_i.
+  wp_auto.
+  wp_apply (wp_shouldOrphanDependents with
+    "[$Hdeepown_m_l $Hdeepown_options_l]").
+  { iFrame "#". iPureIntro. done. }
+  iIntros (should_orphan) "(-> & Hdeepown_m_l & Hdeepown_options_l)".
+  wp_auto.
+  wp_apply (wp_shouldDeleteDependents with
+    "[$Hdeepown_m_l $Hdeepown_options_l]").
+  { iFrame "#". iPureIntro. done. }
+  iIntros (should_delete) "(-> & Hdeepown_m_l & Hdeepown_options_l)".
+  wp_auto.
+  wp_apply wp_slice_literal_non_nil. iSplitR; first done.
+  iIntros (new_sl_ptr) "(Hnew_sl & Hnew_cap & %Hnew_sl_non_nil)".
+  set (new_sl := slice.mk new_sl_ptr (W64 0) (W64 0)). wp_auto.
+  wp_apply (v1.wp_GetFinalizers_deepown with "[$Hdeepown_m_l]").
+  iIntros (old_sl) "(%Hold_sl_nil & Hold_finalizers)".
+  iAssert ("Hold_sl" ∷ old_sl ↦*{dq} default [] m.(ObjectMetaV.Finalizers') ∗
+      "Hrestore_m" ∷ (old_sl ↦*{dq} default [] m.(ObjectMetaV.Finalizers') -∗
+        ObjectMetaV.deepown_l metadata_l m dq))%I
+    with "[Hold_finalizers]" as "(Hold_sl & Hrestore_m)".
+  { destruct m.(ObjectMetaV.Finalizers') as [finalizers|]
+      eqn:Hfinalizers_eq.
+    - iDestruct "Hold_finalizers" as (cfinalizers)
+        "(Hold_sl & -> & Hrestore_m)".
+      iFrame.
+    - assert (old_sl = slice.nil) as -> by
+        (apply (proj2 Hold_sl_nil); done).
+      simpl. iSplitL ""; first iApply (own_slice_nil (V := go_string) dq).
+      iIntros "_". iFrame. }
+  set (keep := fun finalizer : go_string =>
+    finalizer ≠ delete_orphan_finalizer ∧
+    finalizer ≠ delete_foreground_finalizer).
+  set (old_finalizers := default [] m.(ObjectMetaV.Finalizers')).
+  iDestruct (own_slice_len with "Hold_sl") as %[Hold_sl_len Hold_sl_nonneg].
+  wp_auto.
+  set I := (∃ (i : w64) (f : go_string) (result_sl : slice.t),
+    "Hi" ∷ i_ptr ↦ i ∗
+    "Hf" ∷ f_ptr ↦ f ∗
+    "HnewFinalizers" ∷ newFinalizers_ptr ↦ result_sl ∗
+    "Hresult" ∷ result_sl ↦* filter keep (take (sint.nat i) old_finalizers) ∗
+    "Hresult_cap" ∷ own_slice_cap go_string result_sl (DfracOwn 1) ∗
+    "%Hresult_non_nil" ∷ ⌜ result_sl ≠ slice.nil ⌝ ∗
+    "Hold_sl" ∷ old_sl ↦*{dq} old_finalizers ∗
+    "%Hi_bounds" ∷ ⌜ 0 ≤ sint.Z i ≤ sint.Z old_sl.(slice.len) ⌝)%I.
+  iAssert I with "[i f newFinalizers Hnew_sl Hnew_cap Hold_sl]" as "Hloop".
+  { iExists (W64 0), (zero_val go_string), new_sl. iFrame.
+    iPureIntro. split; [exact Hnew_sl_non_nil|word]. }
+  wp_for "Hloop". wp_if_destruct.
+  - destruct (decide (0 ≤ sint.Z i < sint.Z old_sl.(slice.len)))
+      as [_|Hbounds]; last word.
+    destruct (lookup_lt_is_Some_2 old_finalizers (sint.nat i))
+      as [current Hcurrent_lookup].
+    { rewrite Hold_sl_len. word. }
+    wp_apply (wp_load_slice_index with "[$Hold_sl]"); [word|done|].
+    iIntros "Hold_sl". wp_auto.
+    wp_if_destruct.
+    + iApply wp_for_post_continue. wp_auto.
+      iAssert I with
+        "[Hi Hf HnewFinalizers Hresult Hresult_cap Hold_sl]" as "Hloop".
+      { assert (sint.nat (word.add i (W64 1)) = S (sint.nat i)) as Hnext by word.
+        assert (filter keep [delete_orphan_finalizer] = []) as Hfilter.
+        { apply (@filter_singleton_False go_string keep _
+            delete_orphan_finalizer []).
+          intros [Hneq _]. apply Hneq. done. }
+        assert (filter keep
+            (take (sint.nat (word.add i (W64 1))) old_finalizers) =
+          filter keep (take (sint.nat i) old_finalizers)) as Hresult_eq.
+        { rewrite Hnext
+            (take_S_r _ _ delete_orphan_finalizer Hcurrent_lookup)
+            list.filter_app Hfilter app_nil_r. done. }
+        iExists (word.add i (W64 1)), delete_orphan_finalizer, result_sl.
+        rewrite Hresult_eq. iFrame. iPureIntro.
+        split; [exact Hresult_non_nil|word]. }
+      iFrame.
+    + wp_if_destruct.
+      * iApply wp_for_post_continue. wp_auto.
+        iAssert I with
+          "[Hi Hf HnewFinalizers Hresult Hresult_cap Hold_sl]" as "Hloop".
+        { assert (sint.nat (word.add i (W64 1)) = S (sint.nat i)) as Hnext
+            by word.
+          assert (filter keep [delete_foreground_finalizer] = []) as Hfilter.
+          { apply (@filter_singleton_False go_string keep _
+              delete_foreground_finalizer []).
+            intros [_ Hneq]. apply Hneq. done. }
+          assert (filter keep
+              (take (sint.nat (word.add i (W64 1))) old_finalizers) =
+            filter keep (take (sint.nat i) old_finalizers)) as Hresult_eq.
+          { rewrite Hnext
+              (take_S_r _ _ delete_foreground_finalizer Hcurrent_lookup)
+              list.filter_app Hfilter app_nil_r. done. }
+          iExists (word.add i (W64 1)), delete_foreground_finalizer, result_sl.
+          rewrite Hresult_eq. iFrame. iPureIntro.
+          split; [exact Hresult_non_nil|word]. }
+        iFrame.
+      * wp_apply wp_slice_literal. iSplitR; first done.
+        iIntros (one_sl_ptr) "[Hone_sl _]".
+        set (one_sl := slice.mk one_sl_ptr (W64 1) (W64 1)). wp_auto.
+        wp_apply (wp_slice_append with "[$Hresult $Hresult_cap $Hone_sl]").
+        iIntros (result_sl') "(Hresult & Hresult_cap & _)".
+        iDestruct (own_slice_len with "Hresult") as %[Hresult_sl_len _].
+        assert (result_sl' ≠ slice.nil) as Hresult_sl_non_nil.
+        { intros ->. simpl in Hresult_sl_len.
+          assert (sint.nat (W64 0) = 0%nat) as Hzero by word.
+          rewrite Hzero app_length /= in Hresult_sl_len. lia. }
+        wp_auto. iApply wp_for_post_do. wp_auto.
+        iAssert I with
+          "[Hi Hf HnewFinalizers Hresult Hresult_cap Hold_sl]" as "Hloop".
+        { assert (sint.nat (word.add i (W64 1)) = S (sint.nat i)) as Hnext
+            by word.
+          assert (filter keep [current] = [current]) as Hfilter.
+          { apply (@filter_singleton_True go_string keep _ current []).
+            unfold keep, delete_orphan_finalizer, delete_foreground_finalizer.
+            split; congruence. }
+          assert (filter keep
+              (take (sint.nat (word.add i (W64 1))) old_finalizers) =
+            filter keep (take (sint.nat i) old_finalizers) ++ [current])
+              as Hresult_eq.
+          { rewrite Hnext (take_S_r _ _ current Hcurrent_lookup)
+              list.filter_app Hfilter. done. }
+          iExists (word.add i (W64 1)), current, result_sl'.
+          rewrite Hresult_eq. iFrame. iPureIntro.
+          split; [exact Hresult_sl_non_nil|word]. }
+        iFrame.
+  - assert (sint.nat i = length old_finalizers) as Hi_end.
+    { rewrite Hold_sl_len. word. }
+    assert (take (sint.nat i) old_finalizers = old_finalizers) as Htake_all.
+    { apply take_ge. rewrite Hi_end. lia. }
+    iEval (rewrite Htake_all) in "Hresult".
+    iPoseProof ("Hrestore_m" with "Hold_sl") as "Hdeepown_m_l".
+    rewrite exception_do_unseal /exception_do_def.
+    rewrite exception_seq_unseal /exception.exception_seq_def.
+    wp_pures.
+    set Jorphan := (fun v => ⌜ v = execute_val ⌝ ∗ ∃ result_sl,
+      "HnewFinalizers" ∷ newFinalizers_ptr ↦ result_sl ∗
+      "Hresult" ∷ result_sl ↦*
+        (filter keep old_finalizers ++
+          if delete_should_orphan_dependents m options
+          then [delete_orphan_finalizer] else []) ∗
+      "Hresult_cap" ∷ own_slice_cap go_string result_sl (DfracOwn 1) ∗
+      "%Hresult_non_nil" ∷ ⌜ result_sl ≠ slice.nil ⌝)%I.
+    wp_bind (if: #(delete_should_orphan_dependents m options)
+      then _ else _)%E.
+    iApply (wp_wand _ _ _ Jorphan
+      with "[HnewFinalizers Hresult Hresult_cap]")%I;
+      [destruct (delete_should_orphan_dependents m options)
+        eqn:Hshould_orphan; wp_auto|].
+    { wp_apply wp_slice_literal. iSplitR; first done.
+      iIntros (one_sl_ptr) "[Hone_sl _]".
+      set (one_sl := slice.mk one_sl_ptr (W64 1) (W64 1)). wp_auto.
+      wp_apply (wp_slice_append with "[$Hresult $Hresult_cap $Hone_sl]").
+      iIntros (result_sl') "(Hresult & Hresult_cap & _)". wp_auto.
+      iDestruct (own_slice_len with "Hresult") as %[Hresult_sl_len _].
+      assert (result_sl' ≠ slice.nil) as Hresult_sl_non_nil.
+      { intros ->. simpl in Hresult_sl_len.
+        assert (sint.nat (W64 0) = 0%nat) as Hzero by word.
+        rewrite Hzero app_length /= in Hresult_sl_len. lia. }
+      iSplit; first done. iExists result_sl'.
+      simpl. unfold delete_orphan_finalizer. iFrame "%". iFrame. }
+    { iSplit; first done. iExists result_sl.
+      simpl. rewrite !app_nil_r. iFrame "%". iFrame. }
+    iIntros (?) "(-> & Happend_orphan)". iNamed "Happend_orphan". wp_auto.
+    set Jforeground := (fun v => ⌜ v = execute_val ⌝ ∗ ∃ final_sl,
+      "HnewFinalizers" ∷ newFinalizers_ptr ↦ final_sl ∗
+      "Hnew_finalizers" ∷ final_sl ↦*
+        (filter keep old_finalizers ++
+          (if delete_should_orphan_dependents m options
+           then [delete_orphan_finalizer] else []) ++
+          (if delete_should_delete_dependents m options
+           then [delete_foreground_finalizer] else [])) ∗
+      "Hnew_finalizers_cap" ∷
+        own_slice_cap go_string final_sl (DfracOwn 1) ∗
+      "%Hnew_finalizers_non_nil" ∷ ⌜ final_sl ≠ slice.nil ⌝)%I.
+    rewrite execute_val_unseal /execute_val_def. wp_auto.
+    wp_bind (if: #(delete_should_delete_dependents m options)
+      then _ else _)%E.
+    iApply (wp_wand _ _ _ Jforeground
+      with "[HnewFinalizers Hresult Hresult_cap]")%I;
+      [destruct (delete_should_delete_dependents m options)
+        eqn:Hshould_foreground; wp_auto|].
+    { wp_apply wp_slice_literal. iSplitR; first done.
+      iIntros (one_sl_ptr) "[Hone_sl _]".
+      set (one_sl := slice.mk one_sl_ptr (W64 1) (W64 1)). wp_auto.
+      wp_apply (wp_slice_append with "[$Hresult $Hresult_cap $Hone_sl]").
+      iIntros (final_sl) "(Hnew_finalizers & Hnew_finalizers_cap & _)".
+      iDestruct (own_slice_len with "Hnew_finalizers") as %[Hfinal_sl_len _].
+      assert (final_sl ≠ slice.nil) as Hnew_finalizers_non_nil.
+      { intros ->. simpl in Hfinal_sl_len.
+        assert (sint.nat (W64 0) = 0%nat) as Hzero by word.
+        rewrite Hzero !app_length /= in Hfinal_sl_len. lia. }
+      assert (sint.nat (W64 0) = 0%nat) as Hzero by word.
+      iEval (rewrite Hzero /=) in "Hnew_finalizers".
+      iEval (rewrite -app_assoc) in "Hnew_finalizers".
+      wp_auto. iSplit; first done. iExists final_sl.
+      simpl. unfold delete_foreground_finalizer. iFrame "%". iFrame. }
+    { iSplit; first done. iExists result_sl0.
+      simpl. rewrite !app_nil_r. iFrame "%". iFrame. }
+    iIntros (?) "(-> & Happend_foreground)". iNamed "Happend_foreground".
+    assert (filter keep old_finalizers ++
+        (if delete_should_orphan_dependents m options
+         then [delete_orphan_finalizer] else []) ++
+        (if delete_should_delete_dependents m options
+         then [delete_foreground_finalizer] else []) =
+      delete_finalizers_for_gc m options) as Hnew_finalizers_eq.
+    { rewrite /delete_finalizers_for_gc /keep /old_finalizers. done. }
+    iEval (rewrite Hnew_finalizers_eq) in "Hnew_finalizers".
+    wp_auto.
+    rewrite execute_val_unseal /execute_val_def. wp_auto.
+    wp_bind.
+    wp_apply (v1.wp_GetFinalizers_deepown with "[$Hdeepown_m_l]").
+    iIntros (old_sl') "(%Hold_sl_nil' & Hold_finalizers)".
+    iAssert ("Hold_sl" ∷ old_sl' ↦*{dq} default [] m.(ObjectMetaV.Finalizers') ∗
+        "Hrestore_m" ∷ (old_sl' ↦*{dq} default [] m.(ObjectMetaV.Finalizers') -∗
+          ObjectMetaV.deepown_l metadata_l m dq))%I
+      with "[Hold_finalizers]" as "(Hold_sl & Hrestore_m)".
+    { destruct m.(ObjectMetaV.Finalizers') as [finalizers|]
+        eqn:Hfinalizers_eq.
+      - iDestruct "Hold_finalizers" as (cfinalizers)
+          "(Hold_sl & -> & Hrestore_m)".
+        iFrame.
+      - assert (old_sl' = slice.nil) as -> by
+          (apply (proj2 Hold_sl_nil'); done).
+        simpl. iSplitL ""; first iApply (own_slice_nil (V := go_string) dq).
+        iIntros "_". iFrame. }
+    wp_auto.
+    iDestruct (own_slice_len with "Hold_sl") as
+      %[Hold_sl_len' Hold_sl_nonneg'].
+    iDestruct (own_slice_len with "Hnew_finalizers") as
+      %[Hnew_sl_len Hnew_sl_nonneg].
+    rewrite execute_val_unseal /execute_val_def. wp_auto.
+    wp_if_destruct.
+    2: { assert (delete_finalizers_changed old_finalizers
+        (delete_finalizers_for_gc m options)) as Hchanged.
+      { left. intros Hlength_eq.
+        rewrite Hlength_eq in Hold_sl_len'. word. }
+      assert (delete_should_update_finalizers m options = true) as Hupdate.
+      { rewrite /delete_should_update_finalizers /old_finalizers.
+        apply bool_decide_eq_true_2. exact Hchanged. }
+      iPoseProof ("Hrestore_m" with "Hold_sl") as "Hdeepown_m_l".
+      rewrite return_val_unseal /return_val_def. wp_auto.
+      iApply ("HΦ" $! true final_sl (Some (delete_finalizers_for_gc m options))).
+      rewrite /delete_new_finalizers Hupdate /=.
+      iFrame. iSplit; first done. iSplit; first done.
+      iSplit; first (iPureIntro; by apply delete_finalizers_for_gc_valid).
+      iSplit.
+      { iPureIntro. split.
+        - intros Hnil. exfalso. exact (Hnew_finalizers_non_nil Hnil).
+        - discriminate. }
+      done. }
+    + rewrite execute_val_unseal /execute_val_def. wp_auto.
+      wp_apply wp_map_make1 as (old_set_l) "Hold_set".
+      rewrite execute_val_unseal /execute_val_def. wp_auto.
+      wp_alloc old_f_ptr as "Hold_f". wp_auto.
+      wp_alloc old_i_ptr as "Hold_i". wp_auto.
+      iClear "Hi Hf".
+      set Iold := (∃ (oi : w64) (oval : go_string),
+        "Hi" ∷ old_i_ptr ↦ oi ∗
+        "Hf" ∷ old_f_ptr ↦ oval ∗
+        "HoldSet" ∷ oldSet_ptr ↦ old_set_l ∗
+        "Hold_set" ∷ old_set_l ↦$
+          list_to_map (((fun finalizer => (finalizer, true)) <$>
+            take (sint.nat oi) old_finalizers)) ∗
+        "Hold_sl" ∷ old_sl' ↦*{dq} old_finalizers ∗
+        "%Hi_bounds" ∷ ⌜ 0 ≤ sint.Z oi ≤ sint.Z old_sl'.(slice.len) ⌝)%I.
+      iAssert Iold with "[Hold_i Hold_f oldSet Hold_set Hold_sl]" as "Hloop".
+      { iExists (W64 0), (zero_val go_string). iFrame.
+        iPureIntro. word. }
+      wp_for "Hloop". wp_if_destruct.
+      * destruct (decide (0 ≤ sint.Z oi < sint.Z old_sl'.(slice.len)))
+          as [_|Hbounds].
+        2: { exfalso. apply Hbounds. split; [lia|word]. }
+        destruct (lookup_lt_is_Some_2 old_finalizers (sint.nat oi))
+          as [current Hcurrent_lookup].
+        { rewrite Hold_sl_len'. word. }
+        wp_apply (wp_load_slice_index with "[$Hold_sl]"); [word|done|].
+        iIntros "Hold_sl". wp_auto.
+        rewrite execute_val_unseal /execute_val_def. wp_auto.
+        rewrite execute_val_unseal /execute_val_def. wp_auto.
+        wp_apply (wp_map_insert go.string old_set_l _ current true
+          with "Hold_set").
+        iIntros "Hold_set". wp_auto. iApply wp_for_post_do. wp_auto.
+        iAssert Iold with "[Hi Hf HoldSet Hold_set Hold_sl]" as "Hloop".
+        { iExists (word.add oi (W64 1)), current.
+          assert (sint.nat (word.add oi (W64 1)) = S (sint.nat oi))
+            as Hnext by word.
+          assert (list_to_map (((fun finalizer => (finalizer, true)) <$>
+                take (sint.nat (word.add oi (W64 1))) old_finalizers)) =
+              (<[current := true]>
+                (list_to_map (((fun finalizer => (finalizer, true)) <$>
+                  take (sint.nat oi) old_finalizers)) : gmap go_string bool)))
+            as Hmap_eq.
+          { rewrite Hnext (take_S_r _ _ current Hcurrent_lookup) fmap_app /=.
+            rewrite list_to_map_app /=.
+            set (prefix_map := (list_to_map
+              (((fun finalizer => (finalizer, true)) <$>
+                take (sint.nat oi) old_finalizers)) : gmap go_string bool)).
+            fold prefix_map.
+            rewrite insert_empty.
+            destruct (prefix_map !! current) as [b|] eqn:Hlookup.
+            - assert (b = true) as ->.
+              { apply elem_of_list_to_map_2 in Hlookup.
+                apply list_elem_of_fmap in Hlookup as [x [Heq _]].
+                simpl in Heq. congruence. }
+              rewrite (union_singleton_r _ _ true true Hlookup).
+              by rewrite insert_id.
+            - symmetry. by apply insert_union_singleton_r. }
+          rewrite Hmap_eq. iFrame. iPureIntro. word. }
+        iFrame.
+      * assert (sint.nat oi = length old_finalizers) as Hoi_end.
+        { rewrite Hold_sl_len'. word. }
+        assert (take (sint.nat oi) old_finalizers = old_finalizers)
+          as Htake_old_all.
+        { apply take_ge. rewrite Hoi_end. lia. }
+        iEval (rewrite Htake_old_all) in "Hold_set".
+        rewrite execute_val_unseal /execute_val_def. wp_auto.
+        wp_alloc new_f_ptr as "Hnew_f". wp_auto.
+        wp_alloc new_i_ptr as "Hnew_i". wp_auto.
+        iClear "Hi Hf".
+        set Inew := (∃ (ni : w64) (nval : go_string),
+          "Hi" ∷ new_i_ptr ↦ ni ∗
+          "Hf" ∷ new_f_ptr ↦ nval ∗
+          "HnewFinalizers" ∷ newFinalizers_ptr ↦ final_sl ∗
+          "Hnew_finalizers" ∷ final_sl ↦* delete_finalizers_for_gc m options ∗
+          "Hnew_finalizers_cap" ∷
+            own_slice_cap go_string final_sl (DfracOwn 1) ∗
+          "HoldSet" ∷ oldSet_ptr ↦ old_set_l ∗
+          "Hold_set" ∷ old_set_l ↦$
+            list_to_map (((fun finalizer => (finalizer, true)) <$> old_finalizers)) ∗
+          "Hold_sl" ∷ old_sl' ↦*{dq} old_finalizers ∗
+          "%Hi_bounds" ∷ ⌜ 0 ≤ sint.Z ni ≤ sint.Z final_sl.(slice.len) ⌝ ∗
+          "%Hseen" ∷ ⌜ ∀ finalizer,
+            finalizer ∈ take (sint.nat ni) (delete_finalizers_for_gc m options) →
+            finalizer ∈ old_finalizers ⌝)%I.
+        iAssert Inew with
+          "[Hnew_i Hnew_f HnewFinalizers Hnew_finalizers Hnew_finalizers_cap
+            HoldSet Hold_set Hold_sl]" as "Hloop".
+        { iExists (W64 0), (zero_val go_string). iFrame.
+          iPureIntro. split; [word|]. rewrite take_0. intros ? Hin.
+          apply elem_of_nil in Hin. contradiction. }
+        wp_for "Hloop". wp_if_destruct.
+        -- destruct (decide (0 ≤ sint.Z ni < sint.Z final_sl.(slice.len)))
+             as [_|Hbounds]; last word.
+           destruct (lookup_lt_is_Some_2 (delete_finalizers_for_gc m options)
+             (sint.nat ni)) as [current Hcurrent_lookup].
+           { rewrite Hnew_sl_len. word. }
+           wp_apply (wp_load_slice_index with "[$Hnew_finalizers]"); [word|done|].
+           iIntros "Hnew_finalizers". wp_auto.
+           rewrite execute_val_unseal /execute_val_def. wp_auto.
+           rewrite execute_val_unseal /execute_val_def. wp_auto.
+           wp_apply (wp_map_lookup1 go.string go.bool old_set_l _ current
+             with "Hold_set") as "Hold_set".
+           rewrite delete_finalizer_set_lookup.
+           destruct (decide (current ∈ old_finalizers)) as [Hcurrent_old|Hcurrent_old].
+           ++ rewrite (bool_decide_eq_true_2 _ Hcurrent_old). wp_auto.
+              iApply wp_for_post_do. wp_auto.
+              iAssert Inew with
+                "[Hi Hf HnewFinalizers Hnew_finalizers Hnew_finalizers_cap
+                  HoldSet Hold_set Hold_sl]" as "Hloop".
+              { iExists (word.add ni (W64 1)), current. iFrame.
+                iPureIntro. split; [word|].
+                intros finalizer Hin.
+                assert (sint.nat (word.add ni (W64 1)) =
+                  S (sint.nat ni)) as Hnext by word.
+                rewrite Hnext (take_S_r _ _ current Hcurrent_lookup) in Hin.
+                apply elem_of_app in Hin as [Hin|Hin]; first by apply Hseen.
+                apply list_elem_of_singleton in Hin. subst. exact Hcurrent_old. }
+              iFrame.
+           ++ rewrite (bool_decide_eq_false_2 _ Hcurrent_old). wp_auto.
+              iApply wp_for_post_return.
+              rewrite return_val_unseal /return_val_def.
+              wp_auto.
+              assert (delete_finalizers_changed old_finalizers
+                (delete_finalizers_for_gc m options)) as Hchanged.
+              { right. apply Exists_exists. exists current. split.
+                - apply list_elem_of_In. eapply list_elem_of_lookup_2.
+                  exact Hcurrent_lookup.
+                - exact Hcurrent_old. }
+              assert (delete_should_update_finalizers m options = true) as Hupdate.
+              { rewrite /delete_should_update_finalizers /old_finalizers.
+                apply bool_decide_eq_true_2. exact Hchanged. }
+              iPoseProof ("Hrestore_m" with "Hold_sl") as "Hdeepown_m_l".
+              iApply ("HΦ" $! true final_sl
+                (Some (delete_finalizers_for_gc m options))).
+              rewrite /delete_new_finalizers Hupdate /=.
+              iFrame. iSplit; first done. iSplit; first done.
+              iSplit; first (iPureIntro; by apply delete_finalizers_for_gc_valid).
+              iSplit.
+              { iPureIntro. split.
+                - intros Hnil. exfalso. exact (Hnew_finalizers_non_nil Hnil).
+                - discriminate. }
+              done.
+        -- assert (sint.nat ni = length (delete_finalizers_for_gc m options))
+             as Hi_new_end.
+           { rewrite Hnew_sl_len. word. }
+           assert (∀ finalizer, finalizer ∈ delete_finalizers_for_gc m options →
+             finalizer ∈ old_finalizers) as Hnew_subset.
+           { intros finalizer Hin. apply Hseen.
+             rewrite Hi_new_end. rewrite take_ge; [lia|exact Hin]. }
+           assert (¬ delete_finalizers_changed old_finalizers
+             (delete_finalizers_for_gc m options)) as Hnot_changed.
+           { intros [Hlength_neq|Hexists].
+             - apply Hlength_neq.
+               rewrite Hold_sl_len' Hnew_sl_len e. done.
+             - apply Exists_exists in Hexists as (finalizer & Hin & Hnotin).
+               apply (proj2 (list_elem_of_In _ _)) in Hin.
+               exact (Hnotin (Hnew_subset finalizer Hin)). }
+           assert (delete_should_update_finalizers m options = false) as Hupdate.
+           { rewrite /delete_should_update_finalizers /old_finalizers.
+             apply bool_decide_eq_false_2. exact Hnot_changed. }
+           rewrite execute_val_unseal /execute_val_def. wp_auto.
+           rewrite return_val_unseal /return_val_def. wp_auto.
+           iPoseProof ("Hrestore_m" with "Hold_sl") as "Hdeepown_m_l".
+           iApply ("HΦ" $! false old_sl' m.(ObjectMetaV.Finalizers')).
+           rewrite /delete_new_finalizers Hupdate /=.
+           iFrame. iPureIntro. split; first done.
+           split; first done. split; [exact Hvalid_finalizers|exact Hold_sl_nil'].
+Qed.
+
+Definition delete_zero_finalizers o options : Prop :=
+  match delete_new_finalizers (KObjectV.objectmeta o) options with
+  | None => True
+  | Some fs => fs = []
+  end.
+
+Definition delete_zero_grace_period o options : Prop :=
+  (if delete_graceful o options then
+    match delete_new_grace_period_seconds o options with
+    | Some grace_period => grace_period
+    | None => W64 0
+    end
+  else W64 0) = W64 0.
+
+(*  This captures exactly when the delete path removes [key] from [s.m].
+    Reading [kubernetes_model/apimodel/new.go] top-to-bottom:
+    1. We must not take the earlier "already pending graceful deletion" fast path:
+      [if pendingGraceful { return nil }].
+    2. After GC finalizer processing, the object must have no finalizers left.
+    3. The computed grace period must be zero.
+    When all three hold, the Go code reaches:
+      [if len(metadata.GetFinalizers()) == 0 && gracePeriod == 0 { delete(s.m, key) }] *)
+Definition delete_removes_from_state_map o options : Prop :=
+  delete_pending_graceful o = false ∧
+  delete_zero_finalizers o options ∧
+  delete_zero_grace_period o options.
+
+#[global] Instance delete_zero_finalizers_dec o options :
+    Decision (delete_zero_finalizers o options).
+Proof.
+  unfold delete_zero_finalizers.
+  destruct (delete_new_finalizers (KObjectV.objectmeta o) options) as
+    [finalizers|].
+  - destruct finalizers as [|finalizer finalizers].
+    + left. done.
+    + right. discriminate.
+  - left. done.
+Defined.
+
+#[global] Instance delete_zero_grace_period_dec o options :
+    Decision (delete_zero_grace_period o options).
+Proof.
+  unfold delete_zero_grace_period.
+  destruct (delete_graceful o options).
+  - destruct (delete_new_grace_period_seconds o options) as [grace_period|].
+    + apply _.
+    + left. done.
+  - left. done.
+Defined.
+
+#[global] Instance delete_removes_from_state_map_dec o options :
+    Decision (delete_removes_from_state_map o options).
+Proof.
+  unfold delete_removes_from_state_map.
+  destruct (decide (delete_pending_graceful o = false)) as [Hpending|Hpending].
+  2: { right. intros [Hpending' _]. contradiction. }
+  destruct (decide (delete_zero_finalizers o options)) as [Hfinalizers|Hfinalizers].
+  2: { right. intros [_ [Hfinalizers' _]]. contradiction. }
+  destruct (decide (delete_zero_grace_period o options)) as [Hgrace|Hgrace].
+  - left. done.
+  - right. intros [_ [_ Hgrace']]. contradiction.
+Defined.
+
+Context `{!kubernetesModelG Σ}.
 
 Lemma tombed_uid_delete_eq_used_uid_sub
   (abs_state : gmap KKey.t KObjectV.t) (used_uid tombed_uid : gset types.UID.t) key kobj :
